Phi_System/Fiction_Refinement.thy
@@ -1,5 +1,5 @@
 theory Fiction_Refinement
-  imports PhiSem_Formalization_Tools
+  imports PhiSem_Formalization_Tools Phi_Semantics_Framework.Phi_SemFrame_ex
   abbrevs "<refines>" = "\<r>\<e>\<f>\<i>\<n>\<e>\<s>"
       and "<w.r.t>" = "\<w>.\<r>.\<t>"
 begin
@@ -12,9 +12,9 @@ begin
 
 
 
+(*
 
-
-definition Is_Frame_Proc :: \<open>'ret::VALs proc \<Rightarrow> bool\<close>
+definition Is_Frame_Proc :: \<open>'ret proc \<Rightarrow> bool\<close>
   where \<open>Is_Frame_Proc f \<longleftrightarrow>
     (\<forall>v s s' r. Success v s' \<in> f s \<and> r ## s \<longrightarrow> Success v (r * s') \<in> f (r * s) \<and> r ## s') \<and>
     (\<forall>e s s' r. Abnormal e s' \<in> f s \<and> r ## s \<longrightarrow> Abnormal e (r * s') \<in> f (r * s) \<and> r ## s')\<close>
@@ -36,61 +36,47 @@ lemma
     apply (case_tac x; simp add: Bex_def split_comp_Ex)
     using prems(1) prems(2) apply blast
     using prems(1) by blast .
-    
+*)
 
-definition Transition_of :: \<open>'ret::VALs proc \<Rightarrow> 'ret \<phi>arg + ABNM \<Rightarrow> resource rel\<close>
+(*
+definition Transition_of :: \<open>'ret proc \<Rightarrow> 'ret \<phi>arg + ABNM \<Rightarrow> resource rel\<close>
   where \<open>Transition_of f = (\<lambda>x. case x of Inl v \<Rightarrow> { (s,s'). Success v s' \<in> f s \<and> s \<in> RES.SPACE }
-                                        | Inr e \<Rightarrow> { (s,s'). Abnormal e s' \<in> f s \<and> s \<in> RES.SPACE } )\<close>
+                                        | Inr e \<Rightarrow> { (s,s'). Abnormal e s' \<in> f s \<and> s \<in> RES.SPACE } )\<close> *)
 
-declare [[typedef_overloaded]]
-datatype 'ret eval_stat = Normal \<open>'ret \<phi>arg\<close> | Abnm ABNM | Crash
-declare [[typedef_overloaded = false]]
-
-lemma eval_stat_forall:
-  \<open>All P \<longleftrightarrow> (\<forall>ret. P (Normal ret)) \<and> (\<forall>e. P (Abnm e)) \<and> P Crash\<close>
-  by (metis eval_stat.exhaust)
-
-lemma eval_stat_ex:
-  \<open>Ex P \<longleftrightarrow> (\<exists>ret. P (Normal ret)) \<or> (\<exists>e. P (Abnm e)) \<or> P Crash\<close>
-  by (metis eval_stat.exhaust)
-
-
-definition Transition_of' :: \<open>'ret::VALs proc \<Rightarrow> 'ret eval_stat \<Rightarrow> resource rel\<close>
-  where \<open>Transition_of' f = (\<lambda>x. (case x of Normal v \<Rightarrow> { (s,s'). Success v s' \<in> f s \<and> s \<in> RES.SPACE }
-                                          | Abnm e \<Rightarrow> { (s,s'). Abnormal e s' \<in> f s \<and> s \<in> RES.SPACE }
-                                          | Crash \<Rightarrow> { (s,s'). Invalid \<in> f s \<and> s \<in> RES.SPACE }))\<close>
-
-definition Valid_Transition :: \<open>('ret eval_stat \<Rightarrow> 'a rel) \<Rightarrow> bool\<close>
-  where \<open>Valid_Transition tr \<longleftrightarrow> tr Crash = {}\<close>
-
-
-definition Transition_of_Success :: \<open>'ret::VALs proc \<Rightarrow> 'ret \<phi>arg \<Rightarrow> resource rel\<close>
-  where \<open>Transition_of_Success f = (\<lambda>v. { (s,s'). Success v s' \<in> f s })\<close>
-
-
-
-
-definition Raw_Procedure :: "'ret::VALs proc
+(*
+definition Raw_Procedure :: "'ret proc
                         \<Rightarrow> ('ret \<phi>arg \<Rightarrow> resource rel)
                         \<Rightarrow> bool"
     ("\<r>\<a>\<w> \<p>\<r>\<o>\<c> (2_) \<r>\<e>\<f>\<i>\<n>\<e>\<s> _ " [11,11] 10)
   where "Raw_Procedure f S \<longleftrightarrow> (\<forall>x r. f (r * x) \<subseteq> \<S> (\<lambda>v. { r * y | y. (x,y) \<in> S v }) 0)"
 
-definition Fictional_Refine :: "'ret::VALs proc
+definition Fictional_Refine :: "'ret proc
                         \<Rightarrow> ('ret \<phi>arg \<Rightarrow> fiction rel)
                         \<Rightarrow> bool"
-  where \<open>Fictional_Refine f S \<longleftrightarrow> (\<forall>x r. f (r * x) \<subseteq> \<S> (\<lambda>v. { r * y | y. (x,y) \<in> S v }) 0)\<close>
+  where \<open>Fictional_Refine f S \<longleftrightarrow> (\<forall>x r. f (r * x) \<subseteq> \<S> (\<lambda>v. { r * y | y. (x,y) \<in> S v }) 0)\<close> *)
 
-term Domain
 
-definition Fictional_Forward_Simulation :: \<open>'c rel \<Rightarrow> 'a rel \<Rightarrow> ('a::sep_magma_1,'c::sep_magma_1) interp \<Rightarrow> 'a set \<Rightarrow> bool\<close>
-      ("_ \<r>\<e>\<f>\<i>\<n>\<e>\<s> _ \<w>.\<r>.\<t> _ \<i>\<n> _" [11,11,11] 10)
-  where \<open>(F \<r>\<e>\<f>\<i>\<n>\<e>\<s> G \<w>.\<r>.\<t> T \<i>\<n> D) \<longleftrightarrow> (\<forall>x r R. F `` (R * \<I> T (r * x) \<s>\<u>\<b>\<j> r ## x \<and> x \<in> D) \<subseteq> { y'. \<exists>y. y' \<in> R * \<I> T (r * y) \<and> r ## y \<and> (x,y) \<in> G})\<close>
 
-lemma empty_refines_any[simp]:
-  \<open>{} \<r>\<e>\<f>\<i>\<n>\<e>\<s> Any \<w>.\<r>.\<t> I \<i>\<n> AnyD\<close>
+
+(*
+lemma refinement_frame'':
+  \<open> A \<r>\<e>\<f>\<i>\<n>\<e>\<s> B \<w>.\<r>.\<t> I \<i>\<n> D
+\<Longrightarrow> Id_on R * A \<r>\<e>\<f>\<i>\<n>\<e>\<s> Id_on R * B \<w>.\<r>.\<t> I \<i>\<n> R * D\<close>
+  for B :: \<open>'b::sep_monoid rel\<close>
   unfolding Fictional_Forward_Simulation_def
-  by simp
+  apply (clarsimp simp add: subset_iff \<phi>expns Image_def Bex_def Id_on_iff)
+  subgoal for r R u v u' v' rr a b
+
+lemma refinement_frame':
+  \<open> A \<r>\<e>\<f>\<i>\<n>\<e>\<s> B \<w>.\<r>.\<t> I \<i>\<n> D
+\<Longrightarrow> Id_on UNIV * A = A\<close>
+  unfolding Fictional_Forward_Simulation_def
+  apply (clarsimp simp add: subset_iff \<phi>expns Image_def Bex_def Id_on_iff set_eq_iff; rule)
+   apply clarsimp
+  subgoal for r a b
+
+
+  subgoal for x r R u v rr a' b'
 
 lemma
   \<open>Any \<r>\<e>\<f>\<i>\<n>\<e>\<s> Any \<w>.\<r>.\<t> \<F>_it \<i>\<n> D\<close>
@@ -105,66 +91,88 @@ lemma
   \<open>Any \<r>\<e>\<f>\<i>\<n>\<e>\<s> UNIV \<w>.\<r>.\<t> I\<close>
   unfolding Fictional_Forward_Simulation_def
   apply (clarsimp simp add: subset_iff \<phi>expns Image_def Bex_def Id_on_iff)
-  subgoal for x r R t u v
+  subgoal for x r R t u v *)
 
 
-lemma refinement_frame:
-  \<open> 1 \<in> R
-\<Longrightarrow> A \<r>\<e>\<f>\<i>\<n>\<e>\<s> B \<w>.\<r>.\<t> I
-\<Longrightarrow> A \<r>\<e>\<f>\<i>\<n>\<e>\<s> Id_on R * B \<w>.\<r>.\<t> I\<close>
-  for B :: \<open>'b::sep_monoid rel\<close>
-  unfolding Fictional_Forward_Simulation_def
-  apply (clarsimp simp add: subset_iff \<phi>expns Image_def Bex_def Id_on_iff)
-  by (smt (z3) mult_1_class.mult_1_left mult_1_class.mult_1_right sep_disj_multD2 sep_magma_1_left)
+(*
+lemma
+  \<open>refinement_projection I1 (refinement_projection I2 (UNIV * D)) \<subseteq> refinement_projection (I1 o\<^sub>\<I> I2) D\<close>
+unfolding refinement_projection_def
+  apply (clarsimp simp add: Bex_def set_eq_iff set_mult_expn)
+  subgoal for x u v u' v'
 
-lemma sep_refinement_stepwise:
-  \<open> S1 \<r>\<e>\<f>\<i>\<n>\<e>\<s> S2 \<w>.\<r>.\<t> I1 \<i>\<n> UNIV
-\<Longrightarrow> S2 \<r>\<e>\<f>\<i>\<n>\<e>\<s> S3 \<w>.\<r>.\<t> I2 \<i>\<n> D'
-\<Longrightarrow> S1 \<r>\<e>\<f>\<i>\<n>\<e>\<s> S3 \<w>.\<r>.\<t> (I1 o\<^sub>\<I> I2) \<i>\<n> D'\<close>
-  for S1 :: \<open>'a::sep_monoid rel\<close>
-  and S2 :: \<open>'b::sep_monoid rel\<close>
-  and S3 :: \<open>'c::sep_monoid rel\<close>
-  unfolding Fictional_Forward_Simulation_def interp_comp_\<I>
-  apply (auto simp add: subset_iff Image_def Bex_def \<phi>expns split_option_all)
-  subgoal premises prems for x r R t u v xb
-  proof -
-    have \<open>(\<exists>x. (\<exists>u v. x = u * v \<and> u \<in> R \<and> v \<in> \<I> I1 xb \<and> u ## v) \<and> (x, t) \<in> S1)\<close>
-      apply (rule exI[where x=\<open>u * v\<close>], simp add: prems)
-      using prems(6) prems(7) prems(9) by auto
-    note prems(1)[THEN spec[where x=xb],THEN spec[where x=1],THEN spec[where x=\<open>R\<close>],THEN spec[where x=\<open>t\<close>], simplified,
-          THEN mp, OF this]
-    then show ?thesis
-      apply clarsimp
-      subgoal premises prems2 for y u' v'
-      proof -
-        have \<open>(\<exists>xa. (\<exists>u v. xa = u * v \<and> u \<in> {1} \<and> v \<in> \<I> I2 (r * x) \<and> u ## v) \<and> r ## x \<and> x \<in> D' \<and> (xa, y) \<in> S2)\<close>
-          using prems(3) prems(4) prems(8) prems2(1) by auto
-        note prems(2)[THEN spec[where x=x],THEN spec[where x=r],THEN spec[where x=\<open>{1}\<close>], THEN spec[where x=y],
-                THEN mp, OF this]
-        then show ?thesis
-          apply clarsimp
-          using prems2(3) prems2(4) prems2(5) by auto
-      qed
-      .
-  qed .
+lemma
+  \<open>refinement_projection (I1 o\<^sub>\<I> I2) D \<subseteq> refinement_projection I1 (refinement_projection I2 D)\<close>
+  for I1 :: \<open>('c::sep_monoid, 'a::sep_magma_1) interp\<close>
+  unfolding refinement_projection_def
+  apply (clarsimp simp add: Bex_def set_eq_iff set_mult_expn)
+  subgoal for x x' u v
+    by (metis mult_1_class.mult_1_left sep_magma_1_right) *)
 
-lemma sep_refinement_horizontal_stepwise:
-  \<open> A1 \<r>\<e>\<f>\<i>\<n>\<e>\<s> B1 \<w>.\<r>.\<t> I
-\<Longrightarrow> A2 \<r>\<e>\<f>\<i>\<n>\<e>\<s> B2 \<w>.\<r>.\<t> I
-\<Longrightarrow> A1 O A2 \<r>\<e>\<f>\<i>\<n>\<e>\<s> B1 O B2 \<w>.\<r>.\<t> I\<close>
+
+
+
+(*
+lemma
+  \<open> A1 \<r>\<e>\<f>\<i>\<n>\<e>\<s> B1 \<w>.\<r>.\<t> I \<i>\<n> D1
+\<Longrightarrow> A2 \<r>\<e>\<f>\<i>\<n>\<e>\<s> B2 \<w>.\<r>.\<t> I \<i>\<n> D2
+\<Longrightarrow> A1 * A2 \<r>\<e>\<f>\<i>\<n>\<e>\<s> B1 * B2 \<w>.\<r>.\<t> I \<i>\<n> D1 * D2\<close>
+  for A1 :: \<open>'a::sep_monoid rel\<close>
   unfolding Fictional_Forward_Simulation_def
   apply (clarsimp simp add: \<phi>expns subset_iff Image_def Bex_def)
-  by (smt (z3) relcomp.relcompI
+  subgoal premises prems for r R u v ux a vx b a' b'
+  proof -
+    thm prems(1)[THEN spec[where x=]]
+    thm prems *)
 
+
+
+(*
+lemma
+  \<open>refinement_projection (\<F>_pointwise I) (fun_upd 1 k ` D') = UNIV * fun_upd 1 k ` refinement_projection I D'\<close>
+  unfolding refinement_projection_def
+  apply (clarsimp simp add: set_eq_iff Bex_def set_mult_expn image_iff; rule; clarsimp simp add: times_fun)
+  prefer 2
+  subgoal for x x' u xc *)
+
+
+
+
+
+
+context resource begin
+
+lemma \<phi>R_get_res_transition:
+  \<open> Transition_of' \<phi>R_get_res' ret = Id_on {s. s \<in> SPACE \<and> ret = Normal (\<phi>arg (get s))}\<close>
+  unfolding Transition_of'_def \<phi>R_get_res'_def Return_def det_lift_def
+  by (cases ret; clarsimp simp add: set_eq_iff Id_on_iff; blast)
+
+lemma setter_transition:
+  \<open> (\<forall>m. m \<in>\<^sub>S\<^sub>H domain \<longrightarrow> P m \<longrightarrow> F m \<in>\<^sub>S\<^sub>H domain)
+\<Longrightarrow> Transition_of' (\<phi>R_set_res' F) ret
+ \<subseteq> {(x,y). x \<in> SPACE \<and> (P (get x) \<longrightarrow> y = updt F x \<and> ret = Normal \<phi>V_none)}\<close>
+  unfolding Transition_of'_def \<phi>R_set_res'_def
+  apply (cases ret; auto simp add: set_eq_iff \<phi>V_none_def if_split_mem2)
+  by (metis \<r>_valid_split fun_upd_same fun_upd_upd proj_inj)
+
+lemma setter_valid:
+  \<open>Valid_Proc (\<phi>R_set_res' F)\<close>
+  unfolding Valid_Proc_def \<phi>R_set_res'_def bind_def Return_def det_lift_def
+  by (clarsimp split: option.split)
+
+
+end
 
 context basic_fiction begin
 
-lemma
+context begin
+
+private lemma from_fictional_refinement':
   \<open> Valid_Proc f
-\<Longrightarrow> (\<And>v. Transition_of' f v \<r>\<e>\<f>\<i>\<n>\<e>\<s> S2 v \<w>.\<r>.\<t> R.basic_fiction o\<^sub>\<I> I \<i>\<n> D)
-\<Longrightarrow> Valid_Transition S2
+\<Longrightarrow> (\<And>v. Transition_of' f v \<r>\<e>\<f>\<i>\<n>\<e>\<s> Rel v \<w>.\<r>.\<t> R.basic_fiction o\<^sub>\<I> I \<i>\<n> D)
+\<Longrightarrow> Valid_Transition Rel
 \<Longrightarrow> x \<in> D
-\<Longrightarrow> \<p>\<r>\<o>\<c> f \<lbrace> x \<Ztypecolon> \<phi> Identity \<longmapsto> \<lambda>v. y \<Ztypecolon> \<phi> Identity \<s>\<u>\<b>\<j> y. (x,y) \<in> S2 (Normal v) \<rbrace> \<t>\<h>\<r>\<o>\<w>\<s> (\<lambda>e. y \<Ztypecolon> \<phi> Identity \<s>\<u>\<b>\<j> y. (x,y) \<in> S2 (Abnm e))\<close>
+\<Longrightarrow> \<p>\<r>\<o>\<c> f \<lbrace> x \<Ztypecolon> \<phi> Identity \<longmapsto> \<lambda>v. y \<Ztypecolon> \<phi> Identity \<s>\<u>\<b>\<j> y. (x,y) \<in> Rel (Normal v) \<rbrace> \<t>\<h>\<r>\<o>\<w>\<s> (\<lambda>e. y \<Ztypecolon> \<phi> Identity \<s>\<u>\<b>\<j> y. (x,y) \<in> Rel (Abnm e))\<close>
   unfolding \<phi>Procedure_alt Fictional_Forward_Simulation_def atomize_all Valid_Transition_def
   apply (auto simp add: Image_iff subset_iff Bex_def R.basic_fiction_\<I> \<phi>expns Transition_of'_def
           LooseStateSpec_def split_sum_all INTERP_RES_def interp_split' R.\<r>_valid_split' interp_comp_\<I>
@@ -173,135 +181,442 @@ lemma
     thm prems
     thm prems(4)[THEN spec[where x=v], THEN spec[where x=x], THEN spec[where x=\<open>get r\<close>], THEN spec[where x=\<open>{u}\<close>], THEN spec[where x=\<open>y'\<close>]]
   proof -
-    have [simp]: \<open>R.clean y' \<in> R.SPACE\<close>
-      by (metis (no_types, lifting) R.\<r>_valid_split R.inj.homo_sep_mult_axioms Valid_Proc_def homo_sep_mult.homo_mult prems(1) prems(10) prems(14) prems(15) prems(16) prems(9) times_fupdt_1_apply_sep times_fupdt_1_fupdt_1_sep)
     have t2: \<open>(\<exists>xa. (\<exists>ua v. xa = ua * v \<and> ua \<in> {u} \<and> (\<exists>xa. xa \<in> \<I> I (get r * x) \<and> v = R.mk xa) \<and> ua ## v) \<and>
-      get r ## x \<and> x \<in> D \<and> Success v y' \<in> f xa \<and> R.clean xa \<in> R.SPACE \<and> (\<exists>m. xa R.name = R.inject m \<and> m \<in>\<^sub>S R.domain))\<close>
+      get r ## x \<and> x \<in> D \<and> Success v y' \<in> f xa \<and> R.clean xa \<in> R.SPACE \<and> (\<exists>m. xa R.name = R.inject m \<and> m \<in>\<^sub>S\<^sub>H R.domain))\<close>
       apply (rule exI[where x=\<open>(u * R.mk y)\<close>], simp add: prems R.inj.homo_mult[symmetric] )
-      using prems(12) prems(13) by blast
+      using prems(11) prems(12) by blast
     note prems(4)[THEN spec[where x=v], THEN spec[where x=x], THEN spec[where x=\<open>get r\<close>], THEN spec[where x=\<open>{u}\<close>], THEN spec[where x=\<open>y'\<close>],
             THEN mp, OF this]
     then show ?thesis
     apply clarsimp
     subgoal for yy ya
       apply (rule exI[where x=yy], clarsimp simp add: inj.homo_mult[symmetric] prems prj.homo_mult, rule)
-      apply (metis R.resource_kind_axioms Valid_Proc_def prems(1) prems(15) resource_kind.\<r>_valid_split t2 times_fupdt_1_apply_sep)
-      using prems(11) by blast .
+      apply (metis R.resource_kind_axioms Valid_Proc_def prems(1) prems(14) resource_kind.\<r>_valid_split t2 times_fupdt_1_apply_sep)
+      using prems(10) by blast .
 qed
   subgoal premises prems for r u y v y' rr
   proof -
     thm prems(5)[THEN spec[where x=v], THEN spec[where x=x], THEN spec[where x=\<open>get r\<close>], THEN spec[where x=\<open>{u}\<close>], THEN spec[where x=\<open>y'\<close>]]
-    have [simp]: \<open>R.clean y' \<in> R.SPACE\<close>
-      by (metis R.\<r>_valid_split R.inj.homo_mult Valid_Proc_def prems(1) prems(10) prems(14) prems(15) prems(16) prems(9) times_fupdt_1_apply_sep times_fupdt_1_fupdt_1_sep)
     have t2: \<open>(\<exists>xa. (\<exists>ua v. xa = ua * v \<and> ua \<in> {u} \<and> (\<exists>xa. xa \<in> \<I> I (get r * x) \<and> v = R.mk xa) \<and> ua ## v) \<and>
-      get r ## x \<and> x \<in> D \<and> Abnormal v y' \<in> f xa \<and> R.clean xa \<in> R.SPACE \<and> (\<exists>m. xa R.name = R.inject m \<and> m \<in>\<^sub>S R.domain))\<close>
-      by (metis (no_types, lifting) R.inj.homo_mult fiction_kind.sep_disj_get_name_eq fiction_kind_axioms insert_iff prems(10) prems(12) prems(13) prems(14) prems(15) prems(16) prems(3) prems(7) prems(8) prems(9) times_fupdt_1_apply_sep times_fupdt_1_fupdt_1_sep)
+      get r ## x \<and> x \<in> D \<and> Abnormal v y' \<in> f xa \<and> R.clean xa \<in> R.SPACE \<and> (\<exists>m. xa R.name = R.inject m \<and> m \<in>\<^sub>S\<^sub>H R.domain))\<close>
+      by (metis (no_types, lifting) R.inj.homo_mult fiction_kind.sep_disj_get_name_eq fiction_kind_axioms insert_iff mult_in_sep_homo_set prems(11) prems(12) prems(13) prems(14) prems(15) prems(16) prems(17) prems(3) prems(7) prems(8) prems(9) times_fupdt_1_apply_sep times_fupdt_1_fupdt_1_sep)
     note prems(5)[THEN spec[where x=v], THEN spec[where x=x], THEN spec[where x=\<open>get r\<close>], THEN spec[where x=\<open>{u}\<close>], THEN spec[where x=\<open>y'\<close>],
             THEN mp, OF this]
     then show ?thesis
       apply clarsimp
       subgoal for yy ya
         apply (rule exI[where x=yy], clarsimp simp add: inj.homo_mult[symmetric] prems prj.homo_mult, rule)
-        apply (metis R.resource_kind_axioms Valid_Proc_def prems(1) prems(15) resource_kind.\<r>_valid_split t2 times_fupdt_1_apply_sep)
-        using prems(11) by blast .
+        apply (metis R.\<r>_valid_split Valid_Proc_def prems(1) prems(14) t2 times_fupdt_1_apply_sep)
+        using prems(10) by blast .
   qed
-  by (metis (mono_tags, lifting) R.inj.homo_mult sep_disj_get_name times_fupdt_1_apply_sep times_fupdt_1_fupdt_1_sep)
+  by (metis (no_types, lifting) R.inj.homo_mult mult_in_sep_homo_set sep_disj_get_name times_fupdt_1_apply_sep times_fupdt_1_fupdt_1_sep)
+
+
+lemma from_fictional_refinement:
+  \<open> Valid_Proc f
+\<Longrightarrow> YY = (\<lambda>v. y \<Ztypecolon> \<phi> Identity \<s>\<u>\<b>\<j> y. (x,y) \<in> Rel (Normal v))
+\<Longrightarrow> EE = (\<lambda>e. y \<Ztypecolon> \<phi> Identity \<s>\<u>\<b>\<j> y. (x,y) \<in> Rel (Abnm e))
+\<Longrightarrow> (\<And>v. Transition_of' f v \<r>\<e>\<f>\<i>\<n>\<e>\<s> Rel v \<w>.\<r>.\<t> R.basic_fiction o\<^sub>\<I> I \<i>\<n> D)
+\<Longrightarrow> Valid_Transition Rel
+\<Longrightarrow> x \<in> D
+\<Longrightarrow> \<p>\<r>\<o>\<c> f \<lbrace> x \<Ztypecolon> \<phi> Identity \<longmapsto> YY \<rbrace> \<t>\<h>\<r>\<o>\<w>\<s> EE\<close>
+  using from_fictional_refinement' by blast
+
+end
+
+lemma "__getter_rule__":
+  \<open> Valid_Proc getter
+\<Longrightarrow> (\<And>ret. Transition_of' getter ret \<r>\<e>\<f>\<i>\<n>\<e>\<s> Id_on ({x} \<s>\<u>\<b>\<j> ret = Normal (\<phi>arg v)) \<w>.\<r>.\<t> R.basic_fiction o\<^sub>\<I> I \<i>\<n> {x})
+\<Longrightarrow> \<p>\<r>\<o>\<c> getter \<lbrace> x \<Ztypecolon> \<phi> Identity \<longmapsto> \<lambda>ret. x \<Ztypecolon> \<phi> Identity \<s>\<u>\<b>\<j> ret = \<phi>arg v \<rbrace>\<close>
+  by (rule from_fictional_refinement[where Rel = \<open>\<lambda>ret. Id_on ({x} \<s>\<u>\<b>\<j> ret = Normal (\<phi>arg v))\<close>
+                                       and D = \<open>{x}\<close>],
+     assumption,
+     clarsimp simp add: set_eq_iff Subjection_expn Id_on_iff ExSet_expn,
+     simp add: Id_on_iff zero_set_def zero_fun_def,
+     assumption,
+     simp add: Valid_Transition_def zero_set_def,
+     simp)
+
+lemma "__setter_rule__":
+  \<open> Valid_Proc setter
+\<Longrightarrow> (\<And>ret. Transition_of' setter ret \<r>\<e>\<f>\<i>\<n>\<e>\<s> {(x,y)} \<s>\<u>\<b>\<j> ret = Normal \<phi>V_none
+            \<w>.\<r>.\<t> R.basic_fiction o\<^sub>\<I> I \<i>\<n> {x})
+\<Longrightarrow> \<p>\<r>\<o>\<c> setter \<lbrace> x \<Ztypecolon> \<phi> Identity \<longmapsto> \<lambda>_. y \<Ztypecolon> \<phi> Identity \<rbrace>\<close>
+  by (rule from_fictional_refinement
+                  [where Rel=\<open>\<lambda>ret. {(x,y)} \<s>\<u>\<b>\<j> ret = Normal \<phi>V_none\<close> and D = \<open>{x}\<close>],
+      assumption,
+      clarsimp simp add: set_eq_iff Subjection_expn Id_on_iff ExSet_expn \<phi>arg_All fun_eq_iff \<phi>V_none_def,
+      simp add: Id_on_iff zero_set_def zero_fun_def,
+      assumption,
+      simp add: Valid_Transition_def zero_set_def,
+      simp)
+
+lemma "__allocator_rule__":
+  \<open> Valid_Proc allocator
+\<Longrightarrow> (\<And>ret. Transition_of' allocator ret \<r>\<e>\<f>\<i>\<n>\<e>\<s> {(1,y k)} \<s>\<u>\<b>\<j> k. ret = Normal (\<phi>arg k) \<and> P k
+            \<w>.\<r>.\<t> R.basic_fiction o\<^sub>\<I> I \<i>\<n> {1})
+\<Longrightarrow> \<p>\<r>\<o>\<c> allocator \<lbrace> Void \<longmapsto> \<lambda>ret. y k \<Ztypecolon> \<phi> Identity \<s>\<u>\<b>\<j> k. ret = \<phi>arg k \<and> P k \<rbrace>\<close>
+  by (rule from_fictional_refinement
+        [where Rel=\<open>\<lambda>ret. {(1,y k)} \<s>\<u>\<b>\<j> k. ret = Normal (\<phi>arg k) \<and> P k\<close>
+           and x=\<open>1\<close> and D=\<open>{1}\<close>, unfolded \<phi>_unit],
+      assumption,
+      clarsimp simp add: set_eq_iff Subjection_expn Id_on_iff ExSet_expn \<phi>arg_All fun_eq_iff \<phi>V_none_def,
+      simp add: Id_on_iff zero_set_def zero_fun_def,
+      assumption,
+      simp add: Valid_Transition_def zero_set_def,
+      simp)
+end
+
+
+subsubsection \<open>2-level Partial Map Resource\<close>
+
+context partial_map_resource2 begin
+
+lemma getter_transition:
+  \<open> Transition_of' (\<phi>R_get_res_entry' k k2) ret
+        = Id_on {s. s \<in> SPACE \<and> ret = (case get s k k2 of Some v \<Rightarrow> Normal (\<phi>arg v) | _ \<Rightarrow> Crash)}\<close>
+  unfolding Transition_of'_def \<phi>R_get_res'_def \<phi>R_get_res_entry'_def bind_def Return_def det_lift_def
+  by (cases ret; clarsimp simp add: set_eq_iff Id_on_iff split: option.split; blast)
+
+lemma getter_refinement:
+  \<open>Transition_of' (\<phi>R_get_res_entry' k k2) ret
+   \<r>\<e>\<f>\<i>\<n>\<e>\<s> Id_on ({1(k := 1(k2 \<mapsto> any))} \<s>\<u>\<b>\<j> ret = Normal (\<phi>arg any))
+   \<w>.\<r>.\<t> basic_fiction \<i>\<n> {1(k := 1(k2 \<mapsto> any))}\<close>
+  unfolding Fictional_Forward_Simulation_def getter_transition
+  apply (cases ret; clarsimp split: option.split simp add: basic_fiction_\<I> set_mult_expn Id_on_iff
+          Subjection_expn zero_set_def set_eq_iff prj.homo_mult times_fun)
+  by (smt (verit, del_insts) fun_sep_disj_imply_v fun_upd_triv mult_1_class.mult_1_right option.exhaust option.inject sep_disj_commuteI sep_disj_get_name sep_disj_multD2 sep_disj_option_nonsepable(2) sep_mult_commute)
+  
+lemma getter_valid:
+  \<open>Valid_Proc (\<phi>R_get_res_entry' k k2)\<close>
+  unfolding Valid_Proc_def \<phi>R_get_res_entry'_def \<phi>R_get_res'_def bind_def Return_def det_lift_def
+  by (clarsimp split: option.split)
+
+
+lemma setter_refinement:
+  \<open> \<forall>m. m \<in>\<^sub>S\<^sub>H domain \<longrightarrow> m k k2 = Some any \<longrightarrow> map_fun_at (map_fun_at (\<lambda>_. u) k2) k m \<in>\<^sub>S\<^sub>H domain
+\<Longrightarrow> Transition_of' (\<phi>R_set_res' (map_fun_at (map_fun_at (\<lambda>_. u) k2) k)) ret
+\<r>\<e>\<f>\<i>\<n>\<e>\<s> pairself (fun_upd 1 k) ` pairself (fun_upd 1 k2) ` {(Some any, u)} \<s>\<u>\<b>\<j> ret = Normal \<phi>V_none
+\<w>.\<r>.\<t> basic_fiction \<i>\<n> (fun_upd 1 k) ` (fun_upd 1 k2) ` {Some any}\<close>
+  apply (rule refinement_sub_fun[OF setter_transition[where F=\<open>map_fun_at (map_fun_at (\<lambda>_. u) k2) k\<close>]], assumption)
+  unfolding Fictional_Forward_Simulation_def setter_transition
+  apply (clarsimp simp add: basic_fiction_\<I> \<phi>expns prj.homo_mult times_fun_upd sep_disj_partial_map_upd
+        nonsepable_semigroup_sepdisj_fun SPACE_mult_homo \<r>_valid_split'
+        times_fun inj.homo_mult[symmetric] inject_wand_homo)
+  subgoal premises prems for r R x' u' a
+  proof -
+    have t1[simp]: \<open>a k k2 ## Some any\<close>
+      by (metis fun_sep_disj_imply_v fun_upd_triv prems(5) prems(9) sep_disj_commuteI sep_disj_multD2)
+    have t2[simp]: \<open>r k k2 ## a k k2 * Some any\<close>
+      by (metis fun_sep_disj_1_fupdt(1) fun_upd_triv nonsepable_semigroup_sepdisj_fun prems(5))
+    have t3[simp]: \<open>r k k2 * (a k k2 * Some any) = Some any\<close>
+      using t1 t2 by force
+    have t4[simp]: \<open>x' = clean u' * mk (map_fun_at (map_fun_at (\<lambda>_. u) k2) k (r * (a * 1(k := 1(k2 \<mapsto> any))))) \<and> ret = Normal \<phi>V_none\<close>
+      using prems(3) by fastforce
+    have t5[simp]: \<open>r ## 1(k := 1(k2 := u))\<close>
+      by (metis fun_sep_disj_1_fupdt(1) fun_upd_triv nonsepable_semigroup_sepdisj_fun prems(5))
+    have t6[simp]: \<open>(r * a) k k2 = None\<close>
+      by (metis sep_disj_multI1 sep_disj_option_nonsepable(1) t1 t2 times_fun)
+    then have [simp]:
+        \<open>map_fun_at (map_fun_at (\<lambda>_. u) k2) k (r * (a * 1(k := 1(k2 \<mapsto> any))))
+            = (r * a) * 1(k := 1(k2 := u))\<close>
+        unfolding map_fun_at_def fun_eq_iff times_fun_def
+        by simp
+    have t1[simp]: \<open>clean u' * mk a = u'\<close>
+      by (metis fun_split_1 prems(8))
+    show ?thesis
+      apply (simp, rule exI[where x=u']; simp add: prems; rule)
+      apply (smt (verit, del_insts) fun_sep_disj_1_fupdt(1) fun_upd_triv inj.homo_mult inj.sep_disj_homo_semi inject_assoc_homo nonsepable_semigroup_sepdisj_fun prems(5) prems(8) prems(9) sep_disj_multD1 sep_disj_multI1 sep_mult_commute sep_space_entry.times_fun_upd sep_space_entry_axioms times_fupdt_1_apply_sep)
+      by (metis (mono_tags, lifting) fun_sep_disj_1_fupdt(1) fun_upd_triv inj.sep_disj_homo_semi nonsepable_semigroup_sepdisj_fun prems(5) prems(8) prems(9) sep_disj_multD1 sep_disj_multI1 sep_disj_multI2)
+  qed .
 
 end
 
 
 
-definition GTS \<comment> \<open>Greatest Transition of a Specification\<close>
-    :: \<open>'a set \<Rightarrow> 'a set \<Rightarrow> ('a \<times> 'a) set\<close> (infix "\<longrightarrow>\<^sub>R" 25)
-    where \<open>GTS P Q = { (x,y) |x y. x \<in> P \<longrightarrow> y \<in> Q }\<close>
+(* lemma \<phi>R_get_res_transition:
+  \<open> (\<And>res. Transition_of' (F res) ret \<subseteq> Id_on (UNIV \<s>\<u>\<b>\<j> res \<in> UNIV * P ret))
+\<Longrightarrow> Transition_of' (\<phi>R_get_res F) ret \<subseteq> Id_on SPACE * Id_on (mk ` P ret)\<close>
+  unfolding Transition_of'_def \<phi>R_get_res_def
+  apply (cases ret; clarsimp simp add: set_eq_iff Id_on_iff subset_iff Subjection_expn image_iff
+            Bex_def set_mult_expn)
+  apply (smt (verit, ccfv_threshold) SPACE_mult_homo fun_sep_disj_1_fupdt(1) fun_split_1 inj_prj_in_SPACE mk_homo_mult sep_disj_clean sep_disj_mk sep_mult_assoc' times_fun_upd
+  apply (smt (verit) SPACE_mult_homo fun_split_1 inj_prj_in_SPACE mk_homo_mult sep_disj_clean sep_disj_mk sep_disj_multI1 sep_mult_assoc'
+  by (smt (z3) SPACE_mult_homo fun_split_1 inj_prj_in_SPACE mk_homo_mult sep_disj_clean sep_disj_mk sep_disj_multI1 sep_mult_assoc'
+*)
+(*
+  term apply (metis \<r>_valid_split fun_split_1 proj_inj sep_disj_clean)
+  apply (metis \<r>_valid_split fun_split_1 proj_inj sep_disj_clean)
+  by (metis sep_disj_clean) *)
 
-lemma GTS_iff[iff]:
-  \<open>(x,y) \<in> (X \<longrightarrow>\<^sub>R Y) \<longleftrightarrow> (x \<in> X \<longrightarrow> y \<in> Y)\<close>
-  unfolding GTS_def by simp
+lemma
+  \<open>pairself (\<lambda>x. 1(k := x)) ` {(Some any, u)} = {(1(k \<mapsto> any), 1(k := u))}\<close>
+  by (clarsimp simp add: set_eq_iff image_iff; blast)
 
+subsubsection \<open>Mapping Resource\<close>
 
+context mapping_resource begin
 
+lemma allocator_transition:
+  \<open> (\<forall>r. r \<in>\<^sub>S\<^sub>H domain \<longrightarrow> (\<exists>k. k \<notin> dom1 r \<and> P k))
+\<Longrightarrow> Transition_of' (\<phi>R_allocate_res_entry' P init) ret
+        \<subseteq> (Id_on SPACE * {(1, mk (1(k := init))) | k. ret = Normal (\<phi>arg k) \<and> P k})\<close>
+  unfolding Transition_of'_def \<phi>R_allocate_res_entry'_def \<phi>R_get_res_def bind_def Return_def
+      det_lift_def \<phi>R_set_res_def Let_def
+  apply (cases ret; clarsimp simp add: zero_set_def set_eq_iff set_mult_expn Subjection_expn Id_on_iff)
+  subgoal premises prems for r
+  proof -
+    thm prems
+    have t1: \<open>get r \<in>\<^sub>S\<^sub>H domain\<close>
+      using get_res_valid_raw prems(3) by blast
+    define kk where \<open>kk = (SOME k. get r k = 1 \<and> P k)\<close>
+    have t2: \<open>\<exists>k. get r k = 1 \<and> P k\<close>
+      using dom1_def prems(1) t1 by fastforce
+    have t3[simp]: \<open>get r kk = 1 \<and> P kk\<close>
+      unfolding kk_def
+      by (insert t2; clarify; rule someI[where P=\<open>\<lambda>k. get r k = 1 \<and> P k\<close>]; blast)
+    note [simp] = kk_def[symmetric]
+    have t4 [simp]: \<open>(get r)(kk := init) = get r * 1(kk := init)\<close>
+      by (simp add: fun_eq_iff)
+    have t5[simp]: \<open>get r ## 1(kk := init)\<close>
+      by (metis fun_sep_disj_1_fupdt(1) fun_upd_triv sep_magma_1_right t3)
+    show ?thesis
+      apply (simp add: fun_eq_iff inj.homo_mult prems)
+      by (metis fun_sep_disj_1_fupdt(1) fun_upd_triv inj.sep_disj_homo_semi inj_prj_in_SPACE prems(3) t5)
+  qed .
 
+lemma allocator_refinement:
+  \<open> \<forall>r. r \<in>\<^sub>S\<^sub>H domain \<longrightarrow> (\<exists>k. k \<notin> dom1 r \<and> P k)
+\<Longrightarrow> Transition_of' (\<phi>R_allocate_res_entry' P init) ret
+   \<r>\<e>\<f>\<i>\<n>\<e>\<s> {(1, 1(k := init))} \<s>\<u>\<b>\<j> k. ret = Normal (\<phi>arg k) \<and> P k
+   \<w>.\<r>.\<t> basic_fiction \<i>\<n> {1}\<close>
+  apply (rule refinement_sub_fun[OF allocator_transition], assumption)
+  unfolding Fictional_Forward_Simulation_def
+  apply (cases ret; clarsimp simp add: set_mult_expn Subjection_expn basic_fiction_\<I>
+      mk_homo_mult)
+  subgoal premises prems for r R u k
+  proof -
+    have [simp]: \<open>r ## 1(k := init)\<close>
+      using prems(4) prems(6) sep_disj_multD2 by blast
+    show ?thesis
+      apply (simp add: mk_homo_mult)
+      using prems(3) prems(4) prems(6) sep_disj_multI2 sep_mult_assoc by blast
+  qed .
+
+lemma allocator_valid:
+  \<open> \<forall>r. r \<in>\<^sub>S\<^sub>H domain \<longrightarrow> (\<exists>k. k \<notin> dom1 r \<and> P k)
+\<Longrightarrow> \<forall>k. P k \<longrightarrow> 1(k := init) \<in>\<^sub>S\<^sub>H domain
+\<Longrightarrow> Valid_Proc (\<phi>R_allocate_res_entry' P init)\<close>
+  unfolding Valid_Proc_def \<phi>R_allocate_res_entry'_def \<phi>R_get_res_def \<phi>R_set_res_def
+            bind_def Return_def det_lift_def Let_def
+  apply (clarsimp split: option.split)
+  subgoal premises prems for r
+  proof -
+    define kk where \<open>kk = (SOME k. get r k = 1 \<and> P k)\<close>
+    have [simp]: \<open>get r kk = 1 \<and> P kk\<close>
+      by (smt (verit, best) dom1_def kk_def mem_Collect_eq prems(1) prems(3) resource.get_res_valid_raw resource_axioms someI)
+    have t1[simp]: \<open>(get r)(kk := init) = get r * 1(kk := init)\<close>
+      by (simp add: fun_eq_iff)
+    have t2[simp]: \<open>get r ## 1(kk := init)\<close>
+      by (simp add: sep_disj_fun_def)
+    have t3[simp]: \<open>r(name := inject ((get r)(kk := init))) = r * mk(1(kk := init))\<close>
+      apply simp using inj.homo_mult prems(3) by force
+    have [simp]: \<open>r ## mk (1(kk := init))\<close>
+      by (metis fun_sep_disj_1_fupdt(1) fun_upd_triv inj.sep_disj_homo_semi inj_prj_in_SPACE prems(3) t2)
+    show ?thesis
+      by (fold kk_def; simp only: t3; simp add: SPACE_mult_homo prems;
+          simp add: SPACE_def prems(2))
+  qed .
+
+end
+
+subsubsection \<open>1-level Partial Map Resource\<close>
 
 context partial_map_resource begin
 
-term \<open>{(x,y). y = updt (\<lambda>f. f(k := u)) x}\<close>
+lemma getter_transition:
+  \<open> Transition_of' (\<phi>R_get_res_entry' k) ret
+        = Id_on {s. s \<in> SPACE \<and> ret = (case get s k of Some v \<Rightarrow> Normal (\<phi>arg v) | _ \<Rightarrow> Crash)}\<close>
+  unfolding Transition_of'_def \<phi>R_get_res'_def \<phi>R_get_res_entry'_def bind_def Return_def det_lift_def
+  by (cases ret; clarsimp simp add: set_eq_iff Id_on_iff split: option.split; blast)
 
-lemma
-  \<open>{(x,y). x \<in> SPACE \<and> y = updt (\<lambda>f. f(k := u)) x}
-\<r>\<e>\<f>\<i>\<n>\<e>\<s> {(1(k \<mapsto> any)) | any. True} \<longrightarrow>\<^sub>R {(1(k := u))} \<w>.\<r>.\<t> basic_fiction \<i>\<n> {(1(k \<mapsto> any)) | any. True}\<close>
-  unfolding Fictional_Forward_Simulation_def
+lemma getter_refinement:
+  \<open>Transition_of' (\<phi>R_get_res_entry' k) ret
+   \<r>\<e>\<f>\<i>\<n>\<e>\<s> Id_on ({1(k \<mapsto> any)} \<s>\<u>\<b>\<j> ret = Normal (\<phi>arg any))
+   \<w>.\<r>.\<t> basic_fiction \<i>\<n> {1(k \<mapsto> any)}\<close>
+  unfolding Fictional_Forward_Simulation_def getter_transition
+  apply (cases ret; clarsimp split: option.split simp add: basic_fiction_\<I> set_mult_expn Id_on_iff
+          Subjection_expn zero_set_def set_eq_iff prj.homo_mult times_fun)
+  by (smt (verit, best) domIff fun_1upd_homo fun_split_1_not_dom fun_upd_same map_upd_eqD1 sep_disj_partial_map_some_none sep_space_entry.sep_disj_get_name sep_space_entry_axioms)
+
+lemma getter_valid:
+  \<open>Valid_Proc (\<phi>R_get_res_entry' k)\<close>
+  unfolding Valid_Proc_def \<phi>R_get_res_entry'_def \<phi>R_get_res'_def bind_def Return_def det_lift_def
+  by (clarsimp split: option.split)
+
+lemma setter_refinement:
+  \<open>(\<forall>m. m \<in>\<^sub>S\<^sub>H domain \<longrightarrow> m k = Some any \<longrightarrow> m(k := u) \<in>\<^sub>S\<^sub>H domain)
+\<Longrightarrow> Transition_of' (\<phi>R_set_res' (\<lambda>f. f(k := u))) ret
+  \<r>\<e>\<f>\<i>\<n>\<e>\<s> pairself (fun_upd 1 k) ` {(Some any, u)} \<s>\<u>\<b>\<j> ret = Normal \<phi>V_none \<w>.\<r>.\<t> basic_fiction \<i>\<n> fun_upd 1 k ` {Some any}\<close>
+  apply (rule refinement_sub_fun[OF setter_transition[where F=\<open>\<lambda>f. f(k := u)\<close>]], assumption)
+  unfolding Fictional_Forward_Simulation_def setter_transition
   apply (clarsimp simp add: basic_fiction_\<I> \<phi>expns prj.homo_mult times_fun_upd sep_disj_partial_map_upd
-        nonsepable_semigroup_sepdisj_fun)
-apply (clarsimp simp add: sep_disj_partial_map_upd
-          nonsepable_semigroup_sepdisj_fun mk_homo_mult)
-  subgoal premises prems for r R u' any
+        nonsepable_semigroup_sepdisj_fun SPACE_mult_homo \<r>_valid_split'
+        times_fun inj.homo_mult[symmetric] inject_wand_homo dom_mult)
+  subgoal premises prems for r R x' u' a
   proof -
-    have [simp]: \<open>(get u' * (r * 1(k \<mapsto> any)))(k := u) = get u' * (r * 1(k := u))\<close>
-      by (metis domIff fun_upd_same fun_upd_upd mk_homo_mult option.distinct(1) prems(2) prems(4) sep_disj_get_name sep_disj_partial_map_upd)
-    have [simp]: \<open>get u' ## (r * 1(k := u))\<close>
-      by (metis mk_homo_mult nonsepable_semigroup_sepdisj_fun prems(2) prems(4) sep_disj_get_name sep_disj_multD1 sep_disj_multI1 sep_disj_multI2)
-    have [simp]: \<open>r ## 1(k := u)\<close>
-      by (meson nonsepable_semigroup_sepdisj_fun prems(2))
-    have [simp]: \<open>r ## (get u' * 1(k := u))\<close>
-      by (metis \<open>get u' ## r * 1(k := u)\<close> \<open>r ## 1(k := u)\<close> sep_disj_commuteI sep_disj_multI1 sep_mult_commute)
-    have [simp]: \<open>get u' ## 1(k := u)\<close>
-      using \<open>get u' ## r * 1(k := u)\<close> \<open>r ## 1(k := u)\<close> sep_disj_commute sep_disj_multD2 by blast
-    have \<open>clean u' * mk(get u') = u'\<close>
-      by (smt (verit, ccfv_threshold) fun_split_1 inj.homo_sep_wand mk_homo_mult prems(1) prems(2) prems(4) resource_kind.inj_prj_in_SPACE resource_kind_axioms sep_insertion.proj_inj sep_insertion_axioms sep_space_entry.sep_disj_mk_name sep_space_entry_axioms times_fupdt_1_apply_sep)
-    show ?thesis
-      apply (simp add: mk_homo_mult)
-      apply (rule exI[where x=u']; rule)
-      apply (smt (verit, best) \<open>clean u' * mk (get u') = u'\<close> \<open>get u' ## r * 1(k := u)\<close> \<open>r ## 1(k := u)\<close> mk_homo_mult sep_disj_clean sep_disj_mk sep_mult_assoc' sep_mult_left_commute)
-      by (metis \<open>clean u' * mk (get u') = u'\<close> \<open>get u' ## r * 1(k := u)\<close> \<open>r ## 1(k := u)\<close> mk_homo_mult prems(3) sep_disj_clean sep_disj_mk sep_disj_multI1)
-  qed
-  .
-      thm mk_homo_mult
-    apply (rule exI[where x=u']; simp add: prems)
-    apply rule
-     prefer 2
-  proof -
-    have t1[simp]: \<open>r ## 1(k := u)\<close>
-      by (meson nonsepable_semigroup_sepdisj_fun prems(1))
-    have t2: \<open>u' ## mk r * mk (1(k \<mapsto> any))\<close>
-      by (metis fun_1upd_homo inj.homo_mult prems(1) prems(3))
-    show \<open>u' ## mk (r * 1(k := u))\<close> 
-     apply (clarsimp simp add: mk_homo_mult)
-      thm mk_homo_mult
-      thm prems[simplified mk_homo_mult]
-
-  subgoal for r R u' any
-proof -
-    have t1: \<open>clean x * mk aa = x\<close>
+    have t1[simp]: \<open>a ## 1(k \<mapsto> any)\<close>
+      using prems(5) prems(9) sep_disj_commuteI sep_disj_multD2 by blast
+    have t2[simp]: \<open>r ## (a * 1(k \<mapsto> any))\<close>
+      by (simp add: prems(5) prems(9) sep_disj_commuteI sep_disj_multI1 sep_mult_commute)
+    have t3[simp]: \<open>x' = clean u' * mk ((r * (a * 1(k \<mapsto> any)))(k := u)) \<and> ret = Normal \<phi>V_none\<close>
+      by (smt (z3) map_upd_Some_unfold prems(3) prems(5) sep_disj_partial_map_some_none t1 times_option(3))
+    have t4[simp]: \<open>mk ((r * (a * 1(k \<mapsto> any)))(k := u)) = mk (r * (a * 1(k := u)))\<close>
+      by (metis domIff fun_upd_same fun_upd_upd option.distinct(1) sep_disj_partial_map_upd t1 t2)
+    have t5[simp]: \<open>clean u' * mk a = u'\<close>
       by (metis fun_split_1 prems(8))
-    have t2: \<open>clean x ## (mk aa * mk (1(k := u)))\<close>
-      by (simp add: fun_1upd_homo)
     show ?thesis
-      by (metis nonsepable_semigroup_sepdisj_fun prems(6) prems(9) sep_disj_mk sep_disj_multI1 sep_mult_assoc' t1 t2)
+      apply (simp add: prems, rule exI[where x=u']; simp add: prems; rule)
+      apply (smt (verit, ccfv_threshold) mk_homo_mult nonsepable_semigroup_sepdisj_fun prems(5) prems(9) sep_disj_clean sep_disj_mk sep_disj_multD1 sep_disj_multI1 sep_disj_multI2 sep_mult_assoc' sep_mult_left_commute t4 t5)
+      by (smt (verit, best) fun_1upd_homo_right1 fun_sep_disj_1_fupdt(1) inj.sep_disj_homo mult_1_class.mult_1_left nonsepable_semigroup_sepdisj_fun sep_disj_commute sep_disj_multD1 sep_disj_multI1 sep_mult_commute t1 t2 t5)
   qed .
-(*\<exists>ub. clean ua * mk ((get ua * (r * 1(k \<mapsto> any)))(k := u)) = ub * mk (r * 1(k := u)) \<and> ub \<in> R \<and> ub ## mk (r * 1(k := u))*)
-(*\<exists>xa. clean x * (mk a * mk (1(k := u))) = xa * mk (1(k := u)) \<and> xa \<in> R \<and> xa ## mk (1(k := u))*)
-  
-    apply rule
-
-  prefer 2
-  apply (meson nonsepable_semigroup_sepdisj_fun)
-  subgoal for x r R u'
-    apply (rule exI[where x=\<open>x(k:=u)\<close>])
-    
-thm sep_disj_partial_map_upd
-
-  unfolding \<phi>R_set_res_def Transition_of'_def
-  apply (cases evs; clarsimp simp add: \<phi>expns Fictional_Forward_Simulation_def basic_fiction_\<I>
-          prj.homo_mult)
-
-lemma
-  \<open>updt (\<lambda>f. f(k := u))\<close>
-
-term updt
-term Id
 
 end
+
+
+subsubsection \<open>pointwise_fiction_for_partial_mapping_resource\<close>
+
+locale pointwise_fiction_for_partial_mapping_resource =
+   R: partial_map_resource Res
++  fiction_kind FIC.DOMAIN INTERPRET Fic \<open>R.basic_fiction o\<^sub>\<I> \<F>_pointwise I\<close>
+for Res :: "('key \<Rightarrow> 'val::nonsepable_semigroup option) resource_entry"
+and I :: \<open>('fic::sep_algebra, 'val option) interp\<close>
+and Fic :: "('key \<Rightarrow> 'fic) fiction_entry"
+begin
+
+sublocale basic_fiction Res \<open>\<F>_pointwise I\<close> ..
+
+lemma getter_rule:
+  \<open> refinement_projection I {x} \<subseteq> UNIV * {Some v}
+\<Longrightarrow> \<p>\<r>\<o>\<c> R.\<phi>R_get_res_entry' k \<lbrace> 1(k := x) \<Ztypecolon> \<phi> Identity \<longmapsto> \<lambda>ret. 1(k := x) \<Ztypecolon> \<phi> Identity \<s>\<u>\<b>\<j> ret = \<phi>arg v \<rbrace>\<close>
+  by (rule "__getter_rule__",
+      rule R.getter_valid,
+      rule sep_refinement_stepwise,
+      rule R.getter_refinement[THEN refinement_frame[where R=UNIV]],
+      unfold Subjection_Id_on Subjection_times,
+      rule refinement_subjection[OF constant_refinement],
+      rule \<F>_pointwise_projection[where D'=\<open>{x}\<close> and D=\<open>{Some v}\<close>, simplified],
+      assumption)
+
+lemma setter_rule:
+  \<open> refinement_projection I {v'} \<subseteq> UNIV * {Some v}
+\<Longrightarrow> Id_on UNIV * {(Some v, u)} \<r>\<e>\<f>\<i>\<n>\<e>\<s> {(v', u')} \<w>.\<r>.\<t> I \<i>\<n> {v'}
+\<Longrightarrow> \<forall>m. m \<in>\<^sub>S\<^sub>H R.domain \<longrightarrow> m k = Some v \<longrightarrow> m(k := u) \<in>\<^sub>S\<^sub>H R.domain
+\<Longrightarrow> \<p>\<r>\<o>\<c> R.\<phi>R_set_res' (\<lambda>f. f(k := u))
+      \<lbrace> 1(k := v') \<Ztypecolon> \<phi> Identity \<longmapsto> 1(k := u') \<Ztypecolon> \<phi> Identity \<rbrace> \<close>
+  by (rule "__setter_rule__",
+      rule R.setter_valid,
+      rule sep_refinement_stepwise[
+        OF R.setter_refinement[THEN refinement_frame[where R=UNIV], unfolded Subjection_times]
+           refinement_subjection[OF \<F>_pointwise_refinement]
+           \<F>_pointwise_projection,
+         where D'1=\<open>{v'}\<close> and B4=\<open>{(v',u')}\<close>, simplified],
+      assumption,
+      assumption,
+      assumption)
+
+declare [[unify_trace_failure]]
+
+lemma
+  \<open> \<forall>k. P k \<longrightarrow> 1(k := u) \<in>\<^sub>S\<^sub>H R.domain
+\<Longrightarrow> \<forall>r. r \<in>\<^sub>S\<^sub>H R.domain \<longrightarrow> (\<exists>k. k \<notin> dom1 r \<and> P k)
+\<Longrightarrow> \<p>\<r>\<o>\<c> R.\<phi>R_allocate_res_entry' P u \<lbrace> Void \<longmapsto> \<lambda>ret. 1(k := u') \<Ztypecolon> \<phi> Identity \<s>\<u>\<b>\<j> k. ret = \<phi>arg k \<and> P k \<rbrace> \<close>
+  apply (rule "__allocator_rule__",
+      rule R.allocator_valid,
+      assumption,
+      assumption)
+thm R.allocator_refinement
+thm "__allocator_rule__"
+
+end
+
+subsubsection \<open>pointwise_fiction_for_two_level_partial_mapping_resource\<close>
+
+locale pointwise_fiction_for_two_level_partial_mapping_resource =
+   R: partial_map_resource2 Res
++  fiction_kind FIC.DOMAIN INTERPRET Fic \<open>R.basic_fiction o\<^sub>\<I> \<F>_pointwise (\<F>_pointwise I)\<close>
+for Res :: "('key \<Rightarrow> 'key2 \<Rightarrow> 'val::nonsepable_semigroup option) resource_entry"
+and I :: \<open>('fic::sep_algebra, 'val option) interp\<close>
+and Fic :: "('key \<Rightarrow> 'key2 \<Rightarrow> 'fic) fiction_entry"
+begin
+
+sublocale basic_fiction Res \<open>\<F>_pointwise (\<F>_pointwise I)\<close> ..
+
+lemma getter_rule:
+  \<open> refinement_projection I {x} \<subseteq> UNIV * {Some v}
+\<Longrightarrow> \<p>\<r>\<o>\<c> R.\<phi>R_get_res_entry' k k2 \<lbrace> 1(k := 1(k2 := x)) \<Ztypecolon> \<phi> Identity \<longmapsto>
+                                    \<lambda>ret. 1(k := 1(k2 := x)) \<Ztypecolon> \<phi> Identity \<s>\<u>\<b>\<j> ret = \<phi>arg v \<rbrace>\<close>
+  by (rule "__getter_rule__",
+      rule R.getter_valid,
+      rule sep_refinement_stepwise,
+      rule R.getter_refinement[THEN refinement_frame[where R=UNIV]],
+      unfold Subjection_Id_on Subjection_times,
+      rule refinement_subjection[OF constant_refinement],
+      rule \<F>_pointwise_projection[where D'=\<open>{1(k2 := x)}\<close> and D=\<open>{1(k2 \<mapsto> v)}\<close>, simplified],
+      rule \<F>_pointwise_projection[where D'=\<open>{x}\<close> and D=\<open>{Some v}\<close>, simplified],
+      assumption)
+
+lemma setter_rule:
+  \<open> refinement_projection I {v'} \<subseteq> UNIV * {Some v}
+\<Longrightarrow> Id_on UNIV * {(Some v, u)} \<r>\<e>\<f>\<i>\<n>\<e>\<s> {(v', u')} \<w>.\<r>.\<t> I \<i>\<n> {v'}
+\<Longrightarrow> \<forall>m. m \<in>\<^sub>S\<^sub>H R.domain \<longrightarrow> m k k2 = Some v \<longrightarrow> map_fun_at (map_fun_at (\<lambda>_. u) k2) k m \<in>\<^sub>S\<^sub>H R.domain
+\<Longrightarrow> \<p>\<r>\<o>\<c> R.\<phi>R_set_res' (map_fun_at (map_fun_at (\<lambda>_. u) k2) k)
+      \<lbrace> 1(k := 1(k2 := v')) \<Ztypecolon> \<phi> Identity \<longmapsto> 1(k := 1(k2 := u')) \<Ztypecolon> \<phi> Identity \<rbrace> \<close>
+  by (rule "__setter_rule__",
+      rule R.setter_valid,
+      rule sep_refinement_stepwise[
+        OF R.setter_refinement[THEN refinement_frame[where R=UNIV], unfolded Subjection_times]
+           refinement_subjection[OF \<F>_pointwise_refinement[OF \<F>_pointwise_refinement]]
+           \<F>_pointwise_projection[OF \<F>_pointwise_projection],
+        where D'2=\<open>{v'}\<close> and B6=\<open>{(v',u')}\<close>, simplified],
+      assumption,
+      assumption,
+      assumption)
+
+end
+
+
+
+
+
+
+print_locale share_fiction_for_partial_mapping_resource
+
+
+locale share_fiction_for_partial_mapping_resource' =
+   pointwise_fiction_for_partial_mapping_resource Res \<open>\<F>_functional to_share\<close> Fic
+for Res :: "('key \<Rightarrow> 'val::nonsepable_semigroup option) resource_entry"
+and Fic :: "('key \<Rightarrow> 'val share option) fiction_entry"
+begin
+
+
+end
+
+
+
+
+
+
+term \<open>(o) f\<close>
+
+term \<open>(o\<^sub>\<I>) I\<close>
+
+lemma
+  \<open>Id_on UNIV * Id_on {u} \<r>\<e>\<f>\<i>\<n>\<e>\<s> Id_on {f u} \<w>.\<r>.\<t> I \<i>\<n> {f u}\<close>
+  unfolding Fictional_Forward_Simulation_def
+  by (clarsimp simp add: Id_on_iff set_mult_expn Subjection_expn; blast)
+
+
 
 
 end
