Phi_Algebras/Phi_Fiction.thy
@@ -1,0 +1,479 @@
+theory Phi_Fiction
+  imports Algebras
+begin
+
+section \<open>Interpretation of Fictional Separation\<close>
+
+subsection \<open>Algebraic Structure\<close>
+
+subsubsection \<open>Auxiliary Helper\<close>
+
+definition \<open>pairself f = (\<lambda>(x,y). (f x, f y))\<close>
+
+lemma pairself[simp]:
+  \<open>pairself f (x,y) = (f x, f y)\<close>
+  unfolding pairself_def by simp
+
+lemma pairself_image_Id_on[simp]:
+  \<open>pairself f ` Id_on S = Id_on (f ` S)\<close>
+  by (clarsimp simp add: set_eq_iff Id_on_iff image_iff Bex_def; blast)
+
+
+subsubsection \<open>Fictional Interpretation\<close>
+
+text \<open>
+  Referring to Fictional Separation Logic~\cite{FSL}, the interpretation of fictional separation
+  maps a fictional resource to a set of concrete resource.
+  The interpretation can be any map to set that preserves \<open>1\<close>, the unit of the separation algebra.\<close>
+
+definition Interpretation :: "('a::one \<Rightarrow> 'b::one set) \<Rightarrow> bool"
+  where "Interpretation \<I> \<longleftrightarrow> \<I> 1 = 1"
+
+typedef (overloaded) ('a::one,'b::one) interp
+    = \<open>Collect (Interpretation :: ('a \<Rightarrow> 'b set) \<Rightarrow> bool)\<close>
+  morphisms \<I> Interp
+  by (rule exI[where x = \<open>\<lambda>_. 1\<close>]) (simp add:sep_mult_commute Interpretation_def)
+
+text \<open>Type \<open>('a,'b) interp\<close> encapsulating the 1-preserving condition, represents an interpretation.
+\<^const>\<open>\<I>\<close> activates the interpretation; \<^const>\<open>Interp\<close> constructs an interpretation by checking
+the 1-preserving condition.
+\[@{thm Interp_inverse[simplified]}\]\<close>
+
+lemmas Interp_inverse[simp] = Interp_inverse[simplified]
+
+lemma Interp_one[simp]: "\<I> I 1 = 1"
+  using Interpretation_def \<I> by blast
+
+lemma interp_eq_I[intro!]:
+  \<open>\<I> x = \<I> y \<Longrightarrow> x = y\<close>
+  by (simp add: \<I>_inject)
+  
+
+(*
+definition \<I>\<^sub>r\<^sub>e\<^sub>l :: \<open>('a::one,'b::one) interp \<Rightarrow> ('a \<times> 'b) set\<close> 
+  where \<open>\<I>\<^sub>r\<^sub>e\<^sub>l I = {(x,y). y \<in> \<I> I x}\<close> *)
+
+
+subsubsection \<open>Fictional Refinement\<close>
+
+definition Fictional_Forward_Simulation :: \<open>'c rel \<Rightarrow> 'a rel \<Rightarrow> ('a::sep_magma_1,'c::sep_magma_1) interp \<Rightarrow> 'a set \<Rightarrow> bool\<close>
+      ("_/ \<r>\<e>\<f>\<i>\<n>\<e>\<s> _/ \<w>.\<r>.\<t> _/ \<i>\<n> _" [11,11,11] 10)
+  where \<open>(F \<r>\<e>\<f>\<i>\<n>\<e>\<s> G \<w>.\<r>.\<t> T \<i>\<n> D)
+    \<longleftrightarrow> (\<forall>x r R. F `` (R * \<I> T (r * x) \<s>\<u>\<b>\<j> r ## x \<and> x \<in> D) \<subseteq> { y'. \<exists>y. y' \<in> R * \<I> T (r * y) \<and> r ## y \<and> (x,y) \<in> G})\<close>
+
+text \<open>We use relation directly here but doesn't mean we cannot model return value or threw exceptions.
+They can parameterize the relation, as we don't need to (it is not designed to) abstract the values.
+We only relate resources in different abstractions.
+
+\<^prop>\<open>\<And>ret. F ret \<r>\<e>\<f>\<i>\<n>\<e>\<s> G ret \<w>.\<r>.\<t> T \<i>\<n> D\<close>
+\<close>
+
+definition \<open>refinement_projection I D = \<Union> (\<I> I ` (UNIV * D))\<close>
+
+lemma empty_refines_any[simp]:
+  \<open>{} \<r>\<e>\<f>\<i>\<n>\<e>\<s> Any \<w>.\<r>.\<t> I \<i>\<n> D\<close>
+  unfolding Fictional_Forward_Simulation_def
+  by simp
+
+lemma refinement_sub_domain:
+  \<open> D' \<subseteq> D
+\<Longrightarrow> A \<r>\<e>\<f>\<i>\<n>\<e>\<s> B \<w>.\<r>.\<t> I \<i>\<n> D
+\<Longrightarrow> A \<r>\<e>\<f>\<i>\<n>\<e>\<s> B \<w>.\<r>.\<t> I \<i>\<n> D'\<close>
+  unfolding Fictional_Forward_Simulation_def
+  by (clarsimp simp add: Subjection_expn subset_iff Image_def Bex_def Id_on_iff, blast)
+
+lemma refinement_sub_fun:
+  \<open> A' \<subseteq> A
+\<Longrightarrow> A  \<r>\<e>\<f>\<i>\<n>\<e>\<s> B \<w>.\<r>.\<t> I \<i>\<n> D
+\<Longrightarrow> A' \<r>\<e>\<f>\<i>\<n>\<e>\<s> B \<w>.\<r>.\<t> I \<i>\<n> D\<close>
+  unfolding Fictional_Forward_Simulation_def
+  by (clarsimp simp add: Subjection_expn subset_iff Image_def Bex_def Id_on_iff; blast)
+
+lemma refinement_sub_fun_right:
+  \<open> B \<subseteq> B'
+\<Longrightarrow> A \<r>\<e>\<f>\<i>\<n>\<e>\<s> B \<w>.\<r>.\<t> I \<i>\<n> D
+\<Longrightarrow> A \<r>\<e>\<f>\<i>\<n>\<e>\<s> B' \<w>.\<r>.\<t> I \<i>\<n> D\<close>
+  unfolding Fictional_Forward_Simulation_def
+  by (clarsimp simp add: Subjection_expn subset_iff Image_def Bex_def Id_on_iff; blast)
+
+lemma refinement_frame:
+  \<open> A \<r>\<e>\<f>\<i>\<n>\<e>\<s> B \<w>.\<r>.\<t> I \<i>\<n> D
+\<Longrightarrow> A \<r>\<e>\<f>\<i>\<n>\<e>\<s> Id_on R * B \<w>.\<r>.\<t> I \<i>\<n> R * D\<close>
+  for B :: \<open>'b::sep_monoid rel\<close>
+  unfolding Fictional_Forward_Simulation_def
+  apply (clarsimp simp add: subset_iff Subjection_expn set_mult_expn Image_def Bex_def Id_on_iff)
+  by (smt (z3) sep_disj_multD1 sep_disj_multD2 sep_disj_multI1 sep_disj_multI2 sep_mult_assoc')
+
+lemma sep_refinement_horizontal_stepwise:
+  \<open> A1 \<r>\<e>\<f>\<i>\<n>\<e>\<s> B1 \<w>.\<r>.\<t> I \<i>\<n> D
+\<Longrightarrow> A2 \<r>\<e>\<f>\<i>\<n>\<e>\<s> B2 \<w>.\<r>.\<t> I \<i>\<n> D'
+\<Longrightarrow> (B1 `` D \<subseteq> D')
+\<Longrightarrow> A1 O A2 \<r>\<e>\<f>\<i>\<n>\<e>\<s> B1 O B2 \<w>.\<r>.\<t> I \<i>\<n> D\<close>
+  unfolding Fictional_Forward_Simulation_def
+  apply (clarsimp simp add: set_mult_expn Subjection_expn subset_iff Image_def Bex_def)
+  subgoal premises prems for x r R u v y z
+  proof -
+    have \<open>(\<exists>xa. (\<exists>u v. xa = u * v \<and> u \<in> R \<and> v \<in> \<I> I (r * x) \<and> u ## v) \<and> r ## x \<and> x \<in> D \<and> (xa, y) \<in> A1)\<close>
+      using prems(10) prems(4) prems(5) prems(6) prems(8) prems(9) by blast
+    note prems(1)[THEN spec[where x=x], THEN spec[where x=r], THEN spec[where x=R], THEN spec[where x=y],
+          THEN mp, OF this]
+    then show ?thesis
+      apply clarsimp
+      subgoal premises prems2 for y' u' v'
+      proof -
+        have \<open>(\<exists>x. (\<exists>u v. x = u * v \<and> u \<in> R \<and> v \<in> \<I> I (r * y') \<and> u ## v) \<and> r ## y' \<and> y' \<in> D' \<and> (x, z) \<in> A2)\<close>
+          using prems(3) prems(5) prems(7) prems2(1) prems2(2) prems2(3) prems2(4) prems2(5) prems2(6) by blast
+        note prems(2)[THEN spec[where x=y'], THEN spec[where x=r], THEN spec[where x=R], THEN spec[where x=z],
+          THEN mp, OF this]
+        then show ?thesis
+          apply clarsimp
+          using prems2(2) by blast
+      qed .
+  qed .
+
+lemma constant_refinement:
+  \<open>Id_on UNIV * Id_on A \<r>\<e>\<f>\<i>\<n>\<e>\<s> Id_on B \<w>.\<r>.\<t> I \<i>\<n> B\<close>
+  unfolding Fictional_Forward_Simulation_def
+  by (clarsimp simp add: subset_iff Id_on_iff set_mult_expn Subjection_expn times_fun; blast)
+
+lemma refinement_subjection:
+  \<open> A \<r>\<e>\<f>\<i>\<n>\<e>\<s> B \<w>.\<r>.\<t> I \<i>\<n> D
+\<Longrightarrow> A \<s>\<u>\<b>\<j> P \<r>\<e>\<f>\<i>\<n>\<e>\<s> B \<s>\<u>\<b>\<j> P \<w>.\<r>.\<t> I \<i>\<n> D\<close>
+  unfolding Fictional_Forward_Simulation_def
+  by (clarsimp simp add: Subjection_expn subset_iff Image_def Bex_def Id_on_iff)
+
+lemma refinement_ExSet:
+  \<open> (\<And>v. A v \<r>\<e>\<f>\<i>\<n>\<e>\<s> B v \<w>.\<r>.\<t> I \<i>\<n> D)
+\<Longrightarrow> ExSet A \<r>\<e>\<f>\<i>\<n>\<e>\<s> ExSet B \<w>.\<r>.\<t> I \<i>\<n> D\<close>
+  unfolding Fictional_Forward_Simulation_def
+  by (clarsimp simp add: ExSet_expn subset_iff Image_def Bex_def Id_on_iff, blast)
+
+
+subsection \<open>Instances\<close>
+
+subsubsection \<open>Identity\<close>
+
+definition [simp]: "\<F>_it' x = {x}"
+
+definition "\<F>_it = Interp \<F>_it'"
+
+lemma \<F>_it_\<I>[simp]: "\<I> \<F>_it = \<F>_it'"
+  unfolding \<F>_it_def
+  by (rule Interp_inverse) (simp add: Interpretation_def one_set_def)
+
+lemma \<F>_it_refinement_projection:
+  \<open>refinement_projection \<F>_it S \<subseteq> UNIV * S\<close>
+  unfolding refinement_projection_def
+  by (clarsimp simp add: set_mult_expn)
+
+lemma \<F>_it_refinement:
+  \<open>Id_on UNIV * {(u,v)} \<r>\<e>\<f>\<i>\<n>\<e>\<s> {(u,v)} \<w>.\<r>.\<t> \<F>_it \<i>\<n> {u}\<close>
+  for u :: \<open>'a::{sep_cancel,sep_monoid}\<close>
+  unfolding Fictional_Forward_Simulation_def
+  by (clarsimp simp add: Subjection_expn set_mult_expn,
+      metis sep_cancel sep_disj_multD1 sep_disj_multD2 sep_disj_multI1 sep_disj_multI2 sep_mult_assoc')
+
+
+subsubsection \<open>Composition\<close>
+
+definition interp_comp :: \<open>('b::one,'c::one) interp \<Rightarrow> ('a::one,'b) interp \<Rightarrow> ('a,'c) interp\<close> (infixr "\<circ>\<^sub>\<I>" 55)
+  where \<open>(I1 \<circ>\<^sub>\<I> I2) = Interp (\<lambda>x. \<Union>(\<I> I1 ` \<I> I2 x))\<close>
+
+notation interp_comp  (infixl "o\<^sub>\<I>" 55)
+
+lemma interp_comp_\<I>[simp]:
+  \<open>\<I> (I1 \<circ>\<^sub>\<I> I2) = (\<lambda>x. \<Union>(\<I> I1 ` \<I> I2 x))\<close>
+  unfolding interp_comp_def
+  by (rule Interp_inverse)  (simp add: Interpretation_def one_set_def)
+
+lemma interp_comp_assoc:
+  \<open>(I1 \<circ>\<^sub>\<I> I2) \<circ>\<^sub>\<I> I3 = I1 \<circ>\<^sub>\<I> (I2 \<circ>\<^sub>\<I> I3)\<close>
+  by (subst \<I>_inject[symmetric]; simp)
+
+lemma \<F>_it_comp[simp]:
+  \<open>\<F>_it o\<^sub>\<I> I = I\<close> \<open>I o\<^sub>\<I> \<F>_it = I\<close>
+  by (subst \<I>_inject[symmetric], simp)+
+
+lemma sep_refinement_stepwise:
+  \<open> S1 \<r>\<e>\<f>\<i>\<n>\<e>\<s> S2 \<w>.\<r>.\<t> I1 \<i>\<n> D
+\<Longrightarrow> S2 \<r>\<e>\<f>\<i>\<n>\<e>\<s> S3 \<w>.\<r>.\<t> I2 \<i>\<n> D'
+\<Longrightarrow> refinement_projection I2 D' \<subseteq> D
+\<Longrightarrow> S1 \<r>\<e>\<f>\<i>\<n>\<e>\<s> S3 \<w>.\<r>.\<t> (I1 o\<^sub>\<I> I2) \<i>\<n> D'\<close>
+  unfolding Fictional_Forward_Simulation_def interp_comp_\<I> refinement_projection_def
+  apply (auto simp add: subset_iff Image_def Bex_def Subjection_expn set_mult_expn split_option_all)
+  subgoal premises prems for x r R t u v xb
+  proof -
+    thm prems
+    thm prems(1)[THEN spec[where x=xb],THEN spec[where x=1],THEN spec[where x=\<open>R\<close>],THEN spec[where x=\<open>t\<close>]]
+    have \<open>(\<exists>x. (\<exists>u v. x = u * v \<and> u \<in> R \<and> v \<in> \<I> I1 (1 * xb) \<and> u ## v) \<and> 1 ## xb \<and> xb \<in> D \<and> (x, t) \<in> S1)\<close>
+      apply (simp add: prems)
+      using prems(10) prems(3) prems(4) prems(5) prems(6) prems(7) prems(8) prems(9) by blast
+    note prems(1)[THEN spec[where x=xb],THEN spec[where x=1],THEN spec[where x=\<open>R\<close>],THEN spec[where x=\<open>t\<close>],
+          THEN mp, OF this]
+    then show ?thesis
+      apply clarsimp
+      subgoal premises prems2 for y u'' v''
+      proof -
+        have \<open>(\<exists>xa. (\<exists>u v. xa = u * v \<and> u \<in> {1} \<and> v \<in> \<I> I2 (r * x) \<and> u ## v) \<and> r ## x \<and> x \<in> D' \<and> (xa, y) \<in> S2)\<close>
+          by (simp, rule exI[where x=xb], simp add: prems2 prems)
+        note prems(2)[THEN spec[where x=x],THEN spec[where x=r],THEN spec[where x=\<open>{1}\<close>], THEN spec[where x=y],
+                THEN mp, OF this]
+        then show ?thesis
+          apply clarsimp
+          using prems2(3) prems2(4) prems2(5) by auto
+      qed .
+  qed .
+
+lemma sep_refinement_stepwise':
+  \<open> S1 \<r>\<e>\<f>\<i>\<n>\<e>\<s> S2 \<w>.\<r>.\<t> I1 \<i>\<n> D
+\<Longrightarrow> S2' \<r>\<e>\<f>\<i>\<n>\<e>\<s> S3 \<w>.\<r>.\<t> I2 \<i>\<n> D'
+\<Longrightarrow> refinement_projection I2 D' \<subseteq> D
+\<Longrightarrow> S2 \<subseteq> S2'
+\<Longrightarrow> S1 \<r>\<e>\<f>\<i>\<n>\<e>\<s> S3 \<w>.\<r>.\<t> (I1 o\<^sub>\<I> I2) \<i>\<n> D'\<close>
+  using refinement_sub_fun sep_refinement_stepwise
+  by metis
+
+
+
+subsubsection \<open>Function, pointwise\<close>
+
+definition "\<F>_fun' I = Interp (\<lambda>f. prod (\<lambda>x. \<I> (I x) (f x)) (dom1 f))"
+
+lemma \<F>_fun'_\<I>[simp]: "\<I> (\<F>_fun' I) = (\<lambda>f. prod (\<lambda>x. \<I> (I x) (f x)) (dom1 f))"
+  unfolding \<F>_fun'_def by (rule Interp_inverse) (simp add: Interpretation_def)
+
+lemma \<F>_fun'_split:
+  " finite (dom1 f)
+\<Longrightarrow> \<I> (\<F>_fun' I) f = \<I> (\<F>_fun' I) (f(k:=1)) * \<I> (I k) (f k)
+   \<and> \<I> (\<F>_fun' I) (f(k:=1)) ## \<I> (I k) (f k)"
+  for f :: "'a \<Rightarrow> 'b::sep_algebra"
+  by simp (smt (verit, best) Interp_one dom1_upd fun_upd_triv mult.comm_neutral mult.commute prod.insert_remove)
+
+
+definition "\<F>_fun I = \<F>_fun' (\<lambda>_. I)"
+
+lemma \<F>_fun_\<I>[simp]: "\<I> (\<F>_fun I) = (\<lambda>f. prod (\<I> I o f) (dom1 f))"
+  unfolding \<F>_fun_def by simp
+
+lemma \<F>_fun_split:
+  " finite (dom1 f)
+\<Longrightarrow> \<I> (\<F>_fun I) f = \<I> (\<F>_fun I) (f(k:=1)) * \<I> I (f k)
+  \<and> \<I> (\<F>_fun I) (f(k:=1)) ## \<I> I (f k)"
+  for f :: "'a \<Rightarrow> 'b::sep_algebra"
+  unfolding \<F>_fun_def using \<F>_fun'_split .
+
+lemma \<F>_interp_fun_\<I>_1_fupdt[simp]: "\<I> (\<F>_fun I) (1(k:=v)) = \<I> I v" by simp
+
+
+definition "\<F>_pointwise I = Interp (\<lambda>f. {g. \<forall>x. g x \<in> \<I> I (f x) })"
+
+lemma \<F>_pointwise_\<I>[simp]:
+  "\<I> (\<F>_pointwise I) = (\<lambda>f. {g. \<forall>x. g x \<in> \<I> I (f x) })"
+  unfolding \<F>_pointwise_def
+  by (rule Interp_inverse) (auto simp add: Interpretation_def one_fun_def fun_eq_iff)
+
+lemma \<F>_pointwise_\<F>_it:
+  \<open>\<F>_pointwise \<F>_it = \<F>_it\<close>
+  by (rule interp_eq_I; simp add: fun_eq_iff set_eq_iff)
+
+definition "\<F>_pointwise' I = Interp (\<lambda>f. {g. \<forall>x. g x \<in> \<I> (I x) (f x) })"
+
+lemma \<F>_pointwise'_\<I>[simp]:
+  "\<I> (\<F>_pointwise' I) = (\<lambda>f. {g. \<forall>x. g x \<in> \<I> (I x) (f x) })"
+  unfolding \<F>_pointwise'_def
+  by (rule Interp_inverse) (auto simp add: Interpretation_def one_fun_def fun_eq_iff)
+
+lemma \<F>_pointwise_projection:
+  \<open> refinement_projection I D' \<subseteq> UNIV * D
+\<Longrightarrow> refinement_projection (\<F>_pointwise I) (fun_upd 1 k ` D') \<subseteq> UNIV * fun_upd 1 k ` D\<close>
+  for D :: \<open>'b::sep_monoid set\<close>
+  apply (clarsimp simp add: subset_iff Bex_def image_iff set_mult_expn times_fun
+            refinement_projection_def)
+  subgoal premises prems for t u xb
+  proof -
+    have t1: \<open>u k ## xb\<close>
+      by (metis fun_upd_same prems(3) sep_disj_fun)
+    have \<open>(\<exists>x. (\<exists>xa. (\<exists>u v. xa = u * v \<and> v \<in> D' \<and> u ## v) \<and> x = \<I> I xa) \<and> t k \<in> x)\<close>
+      by (metis prems(2) prems(4) t1)
+    note prems(1)[THEN spec[where x=\<open>t k\<close>], THEN mp, OF this]
+    then show ?thesis
+      apply clarsimp
+      subgoal premises prems2 for u' v'
+        apply (rule exI[where x=\<open>t(k := u')\<close>], rule exI[where x=\<open>1(k := v')\<close>])
+        by (simp add: fun_eq_iff prems2 sep_disj_fun_def times_fun) .
+  qed .
+
+lemma \<F>_pointwise_refinement:
+  \<open> Id_on UNIV * A \<r>\<e>\<f>\<i>\<n>\<e>\<s> B \<w>.\<r>.\<t> I \<i>\<n> D
+\<Longrightarrow> Id_on UNIV * pairself (fun_upd 1 k) ` A \<r>\<e>\<f>\<i>\<n>\<e>\<s> pairself (fun_upd 1 k) ` B
+    \<w>.\<r>.\<t> \<F>_pointwise I \<i>\<n> fun_upd 1 k ` D\<close>
+  unfolding Fictional_Forward_Simulation_def
+  apply (clarsimp simp add: set_mult_expn Subjection_expn image_iff Image_def subset_iff Bex_def times_fun Id_on_iff)
+  subgoal premises prems for r R u v xb xc a b
+  proof -
+    have t1[simp]: \<open>xc k ## a\<close>
+      by (metis fun_upd_same prems(8) sep_disj_fun)
+    have t2[simp]: \<open>xc k ## b\<close>
+      by (metis fun_upd_same prems(9) sep_disj_fun)
+    have \<open>(\<exists>x. (\<exists>ua v. x = ua * v \<and> ua \<in> {u k} \<and> v \<in> \<I> I (r k * xb) \<and> ua ## v) \<and>
+     r k ## xb \<and>
+     xb \<in> D \<and> (\<exists>a ba aa. x = a * aa \<and> (\<exists>bb. xc k * b = ba * bb \<and> a = ba \<and> (aa, bb) \<in> A \<and> a ## aa \<and> ba ## bb)))\<close>
+      by (simp add: prems,
+          smt (verit, del_insts) fun_upd_same prems(10) prems(2) prems(5) prems(6) prems(7) sep_disj_fun_def t1 t2 times_fun)
+    note prems(1)[THEN spec[where x=xb], THEN spec[where x=\<open>r k\<close>], THEN spec[where x=\<open>{u k}\<close>, THEN spec[where x=\<open>xc k * b\<close>]],
+          THEN mp, OF this]
+    then show ?thesis
+      apply clarsimp
+      subgoal premises prems2 for y v'
+      proof -
+        have t4: \<open>u ## v(k := v')\<close>
+          by (clarsimp simp add: sep_disj_fun_def prems2 prems(7)) (simp add: prems(7))
+        have t3: \<open>xc * 1(k := b) = u * v(k := v')\<close>
+          by (clarsimp simp add: fun_eq_iff times_fun prems2,
+              metis (no_types, opaque_lifting) fun_upd_other mult_1_class.mult_1_right prems(5) times_fun_def)
+        show ?thesis
+          by (rule exI[where x=\<open>1(k := y)\<close>]; simp add: prems prems2; rule,
+               smt (verit, ccfv_threshold) fun_split_1 fun_upd_other fun_upd_same prems(3) prems(6) prems2(4) t3 t4 times_fun,
+               metis fun_sep_disj_1_fupdt(1) fun_upd_triv prems2(1) prems2(2))
+      qed .
+  qed .
+
+subsubsection \<open>Pairwise\<close>
+
+definition "\<F>_pair I1 I2 = Interp (\<lambda>(x,y). \<I> I1 x * \<I> I2 y) "
+
+lemma \<F>_pair_\<I>[simp]: "\<I> (\<F>_pair I1 I2) = (\<lambda>(x,y). \<I> I1 x * \<I> I2 y)"
+  for I1 :: "('a::one,'b::sep_monoid) interp"
+  unfolding \<F>_pair_def
+  by (rule Interp_inverse) (simp add: Interpretation_def one_prod_def)
+
+notation \<F>_pair (infixl "\<bullet>\<^sub>\<F>" 50)
+
+
+subsubsection \<open>Option\<close>
+
+definition "\<F>_option I = Interp (case_option 1 I)"
+
+lemma \<F>_option_\<I>[simp]: "\<I> (\<F>_option I) = (case_option 1 I)"
+  unfolding \<F>_option_def
+  by (rule Interp_inverse) (simp add: Interpretation_def)
+
+
+definition "\<F>_optionwise I = Interp (\<lambda>x. case x of Some x' \<Rightarrow> Some ` I x' | _ \<Rightarrow> {None})"
+
+lemma \<F>_optionwise_\<I>[simp]:
+  "\<I> (\<F>_optionwise I) = (\<lambda>x. case x of Some x' \<Rightarrow> Some ` I x' | _ \<Rightarrow> {None})"
+  unfolding \<F>_optionwise_def
+  by (rule Interp_inverse) (auto simp add: Interpretation_def)
+
+
+(* subsubsection \<open>Partiality\<close>
+
+definition "fine I = Interp (case_fine (\<I> I) {})"
+lemma fine_\<I>[simp]: "\<I> (fine I) = case_fine (\<I> I) {}"
+  unfolding fine_def by (rule Interp_inverse) (simp add: Interpretation_def one_fine_def)
+
+definition "defined I = Interp (\<lambda>x. Fine ` \<I> I x)"
+lemma defined_\<I>[simp]: "\<I> (defined I) = (\<lambda>x. Fine ` \<I> I x)"
+  unfolding defined_def
+  by (rule Interp_inverse) (auto simp add: Interpretation_def one_fine_def)
+
+definition "partialwise I = \<F>_fine (defined I)"
+lemma partialwise_\<I>[simp]: "\<I> (partialwise I) (Fine x) = { Fine y |y. y \<in> \<I> I x }"
+  unfolding partialwise_def by auto
+*)
+
+subsubsection \<open>Functional Fiction\<close>
+
+definition \<open>\<F>_functional \<psi> = Interp (\<lambda>x. {y. x = \<psi> y})\<close>
+
+lemma (in kernel_is_1) \<F>_functional_\<I>[simp]:
+  \<open>\<I> (\<F>_functional \<psi>) = (\<lambda>x. {y. x = \<psi> y})\<close>
+  unfolding \<F>_functional_def
+  by (rule Interp_inverse, simp add: Interpretation_def one_set_def set_eq_iff inj_at_1)
+
+lemma map_option_inj_at_1[simp]:
+  \<open>kernel_is_1 (map_option f)\<close>
+  unfolding one_option_def kernel_is_1_def
+  by (simp add: split_option_all)
+
+lemma (in homo_sep_wand_monoid) \<F>_functional_projection [simp]:
+  \<open>refinement_projection (\<F>_functional \<psi>) (\<psi> ` S) \<subseteq> UNIV * S\<close>
+  unfolding refinement_projection_def
+  by (clarsimp simp add: subset_iff set_mult_expn eq_commute[where a=\<open>\<psi> _\<close>]
+          homo_sep_wand; blast)
+
+lemma kernel_is_1_pointwise[locale_intro,intro!]:
+  \<open>kernel_is_1 \<psi> \<Longrightarrow> kernel_is_1 ((\<circ>) \<psi>)\<close>
+  unfolding kernel_is_1_def by (simp add: fun_eq_iff)
+
+lemma (in kernel_is_1) \<F>_functional_pointwise:
+  \<open>\<F>_functional ((\<circ>) \<psi>) = \<F>_pointwise (\<F>_functional \<psi>)\<close>
+proof -
+  interpret kernel_is_1 \<open>(\<circ>) \<psi>\<close> by intro_locales
+  show ?thesis by (rule interp_eq_I; simp add: fun_eq_iff)
+qed
+
+
+definition "\<F>_share s = (case s of Share w v \<Rightarrow> if w = 1 then {v} else {})"
+
+lemma \<F>_share_\<I>[simp]: "\<F>_share (Share w v) = (if w = 1 then {v} else {})"
+  unfolding \<F>_share_def by simp
+
+(* lemma In_ficion_fine [simp]:
+  \<open>x \<in> (case some_fine of Fine y \<Rightarrow> f y | Undef \<Rightarrow> {})
+        \<longleftrightarrow> (\<exists>y. some_fine = Fine y \<and> x \<in> f y)\<close>
+  by (cases some_fine; simp)
+*)
+
+subsubsection \<open>Agreement\<close>
+
+definition \<open>\<F>_agree = (\<lambda>x. case x of agree x' \<Rightarrow> {x'})\<close>
+
+
+subsection \<open>Refinement of Algebraic Structures\<close>
+
+subsubsection \<open>Cancellative Permission Insertion Homomorphism\<close>
+
+context cancl_perm_ins_homo begin
+
+lemma constant_refinement:
+  \<open>Id_on UNIV * Id_on S \<r>\<e>\<f>\<i>\<n>\<e>\<s> Id_on ((share n o \<psi>) ` S) \<w>.\<r>.\<t> \<F>_functional \<psi> \<i>\<n> (share n o \<psi>) ` S\<close>
+  for S :: \<open>'a::{sep_algebra, sep_cancel} set\<close>
+  unfolding Fictional_Forward_Simulation_def
+  by (clarsimp simp add: Id_on_iff set_mult_expn Subjection_expn; blast)
+
+lemmas constant_refinement_1 = constant_refinement[where S=\<open>{u}\<close> for u, simplified]
+
+lemma refinement_projection:
+  \<open>0 < n \<and> n \<le> 1 \<Longrightarrow> refinement_projection (\<F>_functional \<psi>) ((share n o \<psi>) ` S) \<subseteq> UNIV * S\<close>
+  unfolding refinement_projection_def
+  by (auto simp add: set_mult_expn homo_sep_wand share_sep_wand'; blast)
+
+lemma refinement:
+  \<open>Id_on UNIV * {(u,v)} \<r>\<e>\<f>\<i>\<n>\<e>\<s> pairself \<psi> ` {(u, v)} \<w>.\<r>.\<t> \<F>_functional \<psi> \<i>\<n> \<psi> ` {u}\<close>
+  for u :: \<open>'a::{sep_algebra, sep_cancel}\<close>
+  unfolding Fictional_Forward_Simulation_def
+  apply (clarsimp simp add: Id_on_iff set_mult_expn Subjection_expn homo_sep_wand)
+  subgoal premises prems for R ru r1 r2
+  proof -
+    have t1: \<open>ru * u = (r1 * r2) * u\<close>
+      by (simp add: prems(1) prems(5) prems(6) sep_mult_assoc')
+    have t2: \<open>r1 * r2 ## u\<close>
+      using prems(5) prems(6) sep_disj_multI1 by blast
+    have t3: \<open>ru = r1 * r2\<close>
+      using prems(3) sep_cancel t1 t2 by blast
+    have t4: \<open>r2 ## v\<close>
+      using prems(4) prems(5) prems(6) sep_disj_multD1 sep_disj_multD2 t3 by blast
+    then have t5: \<open>\<psi> r2 ## \<psi> v\<close> by simp
+    show ?thesis
+      apply (simp add: t5)
+      apply (rule exI[where x=r1], rule exI[where x=\<open>r2 * v\<close>], simp add: t3)
+      by (metis local.homo_mult prems(2) prems(4) prems(5) prems(6) sep_disj_multD1 sep_disj_multI2 sep_mult_assoc t3 t4)
+  qed .
+
+end
+
+
+
+end
