Phi_Semantics/PhiSem_Machine_Integer.thy
@@ -543,7 +543,7 @@ lemma [\<phi>reason 50
 
 
 subsubsection \<open>Addition\<close>
-
+ 
 lemma op_add_word_\<phi>app[\<phi>synthesis for _ (100)
                                    and \<open>x \<Ztypecolon> \<v>\<a>\<l> Word('b)\<heavy_comma> y \<Ztypecolon> \<v>\<a>\<l> Word('b)\<close> \<Rightarrow> \<open>\<lambda>v. x + y \<Ztypecolon> _\<close> (1200)]:
   \<open> \<p>\<r>\<o>\<c> op_add LENGTH('b) (\<phi>V_pair vy vx) \<lbrace> x \<Ztypecolon> \<v>\<a>\<l>[vx] Word('b)\<heavy_comma> y \<Ztypecolon> \<v>\<a>\<l>[vy] Word('b) \<longmapsto> \<v>\<a>\<l> x + y \<Ztypecolon> Word('b) \<rbrace>\<close>
