Phi_System/PhiSem_Formalization_Tools2.thy
@@ -1,0 +1,232 @@
+theory PhiSem_Formalization_Tools2
+  imports IDE_CP
+begin
+
+section \<open>Tools for Formalizing Instructions\<close>
+
+named_theorems discharging_semantic_debt
+  \<open>Theorems that discharges or helps to discharge the debt axioms for semantic formalization.\<close>
+
+subsection \<open>Elementary Constructions for Formalizing Instructions\<close>
+
+definition \<phi>M_assert :: \<open>bool \<Rightarrow> unit proc\<close>
+  where \<open>\<phi>M_assert P = (\<lambda>s. if P then Return \<phi>V_none s else {Invalid})\<close>
+
+definition \<phi>M_assume :: \<open>bool \<Rightarrow> unit proc\<close>
+  where \<open>\<phi>M_assume P = (\<lambda>s. if P then Return \<phi>V_none s else {AssumptionBroken})\<close>
+
+definition \<phi>M_getV_raw :: \<open>(VAL \<Rightarrow> 'v) \<Rightarrow> VAL \<phi>arg \<Rightarrow> ('v \<Rightarrow> 'y proc) \<Rightarrow> 'y proc\<close>
+  where \<open>\<phi>M_getV_raw VDT_dest v F = F (VDT_dest (\<phi>arg.dest v))\<close>
+
+definition \<phi>M_getV :: \<open>TY \<Rightarrow> (VAL \<Rightarrow> 'v) \<Rightarrow> VAL \<phi>arg \<Rightarrow> ('v \<Rightarrow> 'y proc) \<Rightarrow> 'y proc\<close>
+  where \<open>\<phi>M_getV TY VDT_dest v F =
+    (\<phi>M_assert (\<phi>arg.dest v \<in> Well_Type TY) \<ggreater> F (VDT_dest (\<phi>arg.dest v)))\<close>
+
+definition \<phi>M_caseV :: \<open>(VAL \<phi>arg \<Rightarrow> ('vr,'ret) proc') \<Rightarrow> (VAL \<times> 'vr::FIX_ARITY_VALs,'ret) proc'\<close>
+  where \<open>\<phi>M_caseV F = (\<lambda>arg. case arg of \<phi>arg (a1,a2) \<Rightarrow> F (\<phi>arg a1) (\<phi>arg a2))\<close>
+
+
+lemma Valid_Proc_\<phi>M_assert[intro!, \<phi>reason 1200]:
+  \<open>Valid_Proc (\<phi>M_assert P)\<close>
+  unfolding Valid_Proc_def \<phi>M_assert_def Return_def det_lift_def
+  by clarsimp
+
+lemma Valid_Proc_\<phi>M_assume[intro!, \<phi>reason 1200]:
+  \<open>Valid_Proc (\<phi>M_assume P)\<close>
+  unfolding Valid_Proc_def \<phi>M_assume_def Return_def det_lift_def
+  by clarsimp
+
+lemma Valid_Proc_\<phi>M_getV_raw[intro!, \<phi>reason 1200]:
+  \<open> (\<And>v. Valid_Proc (F v))
+\<Longrightarrow> Valid_Proc (\<phi>M_getV_raw VDF v F)\<close>
+  unfolding Valid_Proc_def \<phi>M_getV_raw_def
+  by blast
+
+
+subsection \<open>Reasoning for Elementary Constructions\<close>
+
+declare \<phi>SEQ[intro!]
+
+lemma \<phi>M_assert[intro!]:
+  \<open>(Inhabited X \<Longrightarrow> P) \<Longrightarrow> \<p>\<r>\<o>\<c> \<phi>M_assert P \<lbrace> X \<longmapsto> \<lambda>_. X \<rbrace> \<t>\<h>\<r>\<o>\<w>\<s> Any\<close>
+  unfolding \<phi>M_assert_def
+  by (rule \<phi>Inhabited; simp; rule)
+
+lemma \<phi>M_assert_True[simp]:
+  \<open>\<phi>M_assert True = Return \<phi>V_none\<close>
+  unfolding \<phi>M_assert_def by simp
+
+lemma \<phi>M_assert':
+  \<open>P \<Longrightarrow> Q (F args) \<Longrightarrow> Q ((\<phi>M_assert P \<ggreater> F) args)\<close>
+  unfolding \<phi>M_assert_def bind_def Return_def det_lift_def by simp
+
+lemma \<phi>M_assume[intro!]:
+  \<open>(P \<Longrightarrow> \<p>\<r>\<o>\<c> F \<lbrace> X \<longmapsto> Y \<rbrace> \<t>\<h>\<r>\<o>\<w>\<s> E) \<Longrightarrow> \<p>\<r>\<o>\<c> (\<phi>M_assume P \<ggreater> F) \<lbrace> X \<longmapsto> Y \<rbrace> \<t>\<h>\<r>\<o>\<w>\<s> E\<close>
+  unfolding \<phi>Procedure_def \<phi>M_assume_def bind_def Return_def det_lift_def
+  by clarsimp
+
+lemma \<phi>M_assume1[intro!]:
+  \<open>\<p>\<r>\<o>\<c> (\<phi>M_assume P) \<lbrace> Void \<longmapsto> Void \<s>\<u>\<b>\<j> P \<rbrace> \<t>\<h>\<r>\<o>\<w>\<s> E\<close>
+  unfolding \<phi>M_assume_def \<phi>Procedure_def bind_def Return_def det_lift_def
+  by clarsimp
+
+lemma \<phi>M_tail_left:  \<open>\<p>\<r>\<o>\<c> F \<lbrace> 1\<heavy_comma> X \<longmapsto> Y \<rbrace> \<t>\<h>\<r>\<o>\<w>\<s> E \<Longrightarrow> \<p>\<r>\<o>\<c> F \<lbrace> X \<longmapsto> Y \<rbrace> \<t>\<h>\<r>\<o>\<w>\<s> E\<close> by simp
+lemma \<phi>M_tail_right: \<open>\<p>\<r>\<o>\<c> F \<lbrace> X \<longmapsto> \<lambda>v. 1 \<heavy_comma> Y v \<rbrace> \<t>\<h>\<r>\<o>\<w>\<s> E \<Longrightarrow> \<p>\<r>\<o>\<c> F \<lbrace> X \<longmapsto> Y \<rbrace> \<t>\<h>\<r>\<o>\<w>\<s> E\<close> by simp
+lemma \<phi>M_tail_right_right: \<open>\<p>\<r>\<o>\<c> F \<lbrace> X \<longmapsto> \<lambda>v. Y v\<heavy_comma> 1 \<rbrace> \<t>\<h>\<r>\<o>\<w>\<s> E \<Longrightarrow> \<p>\<r>\<o>\<c> F \<lbrace> X \<longmapsto> Y \<rbrace> \<t>\<h>\<r>\<o>\<w>\<s> E\<close> by simp
+lemma \<phi>M_shrink_left:  \<open>\<p>\<r>\<o>\<c> F \<lbrace> X \<longmapsto> Y \<rbrace> \<t>\<h>\<r>\<o>\<w>\<s> E \<Longrightarrow> \<p>\<r>\<o>\<c> F \<lbrace> 1\<heavy_comma> X \<longmapsto> Y \<rbrace> \<t>\<h>\<r>\<o>\<w>\<s> E\<close> by simp
+lemma \<phi>M_shrink_right[intro!]: \<open>\<p>\<r>\<o>\<c> F \<lbrace> X \<longmapsto> Y \<rbrace> \<t>\<h>\<r>\<o>\<w>\<s> E \<Longrightarrow> \<p>\<r>\<o>\<c> F \<lbrace> X \<longmapsto> \<lambda>v. 1\<heavy_comma> Y v \<rbrace> \<t>\<h>\<r>\<o>\<w>\<s> E\<close> by simp
+
+lemma \<phi>M_getV_raw[intro!]:
+   \<open>(v \<in> (x \<Ztypecolon> A) \<Longrightarrow> \<p>\<r>\<o>\<c> F (VDT_dest v) \<lbrace> X \<longmapsto> Y \<rbrace> \<t>\<h>\<r>\<o>\<w>\<s> E  )
+\<Longrightarrow> \<p>\<r>\<o>\<c> \<phi>M_getV_raw VDT_dest (\<phi>arg v) F \<lbrace> X\<heavy_comma> x \<Ztypecolon> Val (\<phi>arg v) A \<longmapsto> Y \<rbrace> \<t>\<h>\<r>\<o>\<w>\<s> E \<close>
+  unfolding \<phi>M_getV_raw_def Premise_def
+  by (clarsimp simp add: \<phi>expns norm_precond_conj)
+
+declare \<phi>M_getV_raw[where X=1, simplified, intro!]
+
+lemma \<phi>M_getV[intro!]:
+   \<open>(v \<in> (x \<Ztypecolon> A) \<Longrightarrow> <\<phi>expn> v \<in> Well_Type TY)
+\<Longrightarrow> (v \<in> (x \<Ztypecolon> A) \<Longrightarrow> \<p>\<r>\<o>\<c> F (VDT_dest v) \<lbrace> X \<longmapsto> Y \<rbrace> \<t>\<h>\<r>\<o>\<w>\<s> E  )
+\<Longrightarrow> \<p>\<r>\<o>\<c> \<phi>M_getV TY VDT_dest (\<phi>arg v) F \<lbrace> X\<heavy_comma> x \<Ztypecolon> Val (\<phi>arg v) A \<longmapsto> Y \<rbrace> \<t>\<h>\<r>\<o>\<w>\<s> E \<close>
+  unfolding \<phi>M_getV_def Premise_def
+  by (clarsimp simp add: \<phi>expns norm_precond_conj)
+
+declare \<phi>M_getV[where X=1, simplified, intro!]
+
+lemma \<phi>M_caseV[intro!]:
+  \<open> \<p>\<r>\<o>\<c> F va vb \<lbrace> X \<longmapsto> Y \<rbrace> \<t>\<h>\<r>\<o>\<w>\<s> E
+\<Longrightarrow> \<p>\<r>\<o>\<c> \<phi>M_caseV F (\<phi>V_pair va vb) \<lbrace> X \<longmapsto> Y \<rbrace> \<t>\<h>\<r>\<o>\<w>\<s> E \<close>
+  unfolding \<phi>M_caseV_def \<phi>V_pair_def by simp
+
+
+subsection \<open>Drop & Duplicate Value\<close>
+
+lemma [\<phi>reason 1200 for \<open>?x \<Ztypecolon> Val ?raw ?T \<i>\<m>\<p>\<l>\<i>\<e>\<s> ?Y \<a>\<n>\<d> ?P @action action_dup\<close>]:
+  \<open>x \<Ztypecolon> Val raw T \<i>\<m>\<p>\<l>\<i>\<e>\<s> x \<Ztypecolon> Val raw T \<heavy_comma> x \<Ztypecolon> Val raw T @action action_dup\<close>
+  unfolding Imply_def Action_Tag_def
+  by (clarsimp simp add: \<phi>expns)
+
+lemma [\<phi>reason 1200 for \<open>?R \<heavy_comma> ?x \<Ztypecolon> Val ?raw ?T \<i>\<m>\<p>\<l>\<i>\<e>\<s> ?Y \<a>\<n>\<d> ?P @action action_drop\<close>]:
+  \<open>Void \<heavy_comma> x \<Ztypecolon> Val raw T \<i>\<m>\<p>\<l>\<i>\<e>\<s> Void @action action_drop\<close>
+  unfolding Imply_def Action_Tag_def
+  by (clarsimp simp add: \<phi>expns)
+
+
+subsection \<open>Abnormal\<close>
+
+definition throw :: \<open>ABNM \<Rightarrow> 'ret proc\<close>
+  where \<open>throw raw = det_lift (Abnormal raw)\<close>
+
+lemma throw_reduce_tail[procedure_simps,simp]:
+  \<open>(throw any \<ggreater> f) = throw any\<close>
+  unfolding throw_def bind_def det_lift_def by simp
+
+lemma "__throw_rule__"[intro!]:
+  \<open> (\<And>a. X a \<i>\<m>\<p>\<l>\<i>\<e>\<s> X' a)
+\<Longrightarrow> \<p>\<r>\<o>\<c> (throw excep :: 'ret proc) \<lbrace> X excep \<longmapsto> Any \<rbrace> \<t>\<h>\<r>\<o>\<w>\<s> X'\<close>
+  unfolding \<phi>Procedure_def subset_iff det_lift_def throw_def Imply_def
+  apply clarsimp
+  by (meson Imply_def View_Shift_def view_shift_by_implication)
+
+lemma throw_\<phi>app:
+  \<open> (\<And>v. Remove_Values (X v) (X' v))
+\<Longrightarrow> \<p>\<r>\<o>\<c> throw excep \<lbrace> X excep \<longmapsto> 0 \<rbrace> \<t>\<h>\<r>\<o>\<w>\<s> X' \<close>
+  unfolding \<phi>Procedure_def subset_iff det_lift_def throw_def Remove_Values_def Imply_def
+  apply clarsimp
+  by (meson Imply_def View_Shift_def view_shift_by_implication)
+
+definition op_try :: "'ret proc \<Rightarrow> (ABNM \<Rightarrow> 'ret proc) \<Rightarrow> 'ret proc"
+  where \<open>op_try f g s = \<Union>((\<lambda>y. case y of Success x s' \<Rightarrow> {Success x s'}
+                                       | Abnormal v s' \<Rightarrow> g v s'
+                                       | AssumptionBroken \<Rightarrow> {AssumptionBroken}
+                                       | NonTerm \<Rightarrow> {NonTerm}
+                                       | Invalid \<Rightarrow> {Invalid}) ` f s)\<close>
+
+lemma "__op_try__"[intro!]:
+  \<open> \<p>\<r>\<o>\<c> f \<lbrace> X \<longmapsto> Y1 \<rbrace> \<t>\<h>\<r>\<o>\<w>\<s> (\<lambda>v. E v)
+\<Longrightarrow> (\<And>v. \<p>\<r>\<o>\<c> g v \<lbrace> E v \<longmapsto> Y2 \<rbrace> \<t>\<h>\<r>\<o>\<w>\<s> E2 )
+\<Longrightarrow> \<p>\<r>\<o>\<c> op_try f g \<lbrace> X \<longmapsto> \<lambda>v. Y1 v + Y2 v \<rbrace> \<t>\<h>\<r>\<o>\<w>\<s> E2  \<close>
+  unfolding op_try_def \<phi>Procedure_def subset_iff
+  apply clarsimp subgoal for comp R x s
+    apply (cases s; simp; cases x; clarsimp simp add: \<phi>expns ring_distribs)
+    subgoal premises prems for a b u v
+      using prems(1)[THEN spec[where x=comp], THEN spec[where x=R]]
+      by (metis (no_types, lifting) INTERP_SPEC LooseStateSpec_expn(1) prems(3) prems(6) prems(7) prems(8) prems(9) set_mult_expn)
+    subgoal premises prems for a b c d u v2 proof -
+      have \<open>Abnormal a b \<in> \<S> (\<lambda>v. INTERP_SPEC (R \<heavy_comma> Y1 v)) (\<lambda>v. INTERP_SPEC (R \<heavy_comma> E v))\<close>
+        using prems(1)[THEN spec[where x=comp], THEN spec[where x=R]]
+        using prems(10) prems(3) prems(7) prems(8) prems(9) by blast
+      note this[simplified]
+      then have \<open>Success c d \<in> \<S> (\<lambda>v. INTERP_SPEC (R \<heavy_comma> Y2 v)) (\<lambda>v. INTERP_SPEC (R \<heavy_comma> E2 v))\<close>
+        using prems(2)[of a, THEN spec[where x=b], THEN spec[where x=R]]
+        by (meson INTERP_SPEC prems(4) set_mult_expn)
+      note this[simplified]
+      then show ?thesis
+        by (metis INTERP_SPEC prems(11) set_mult_expn)
+    qed
+    subgoal premises prems for a b c d u v proof -
+      have \<open>Abnormal a b \<in> \<S> (\<lambda>v. INTERP_SPEC (R \<heavy_comma> Y1 v)) (\<lambda>v. INTERP_SPEC (R \<heavy_comma> E v))\<close>
+        using prems(1)[THEN spec[where x=comp], THEN spec[where x=R]]
+        using prems(10) prems(3) prems(7) prems(8) prems(9) by blast
+      note this[simplified]
+      then have \<open>Abnormal c d \<in> \<S> (\<lambda>v. INTERP_SPEC (R \<heavy_comma> Y2 v)) (\<lambda>v. INTERP_SPEC (R \<heavy_comma> E2 v))\<close>
+        using prems(2)[THEN spec[where x=b], THEN spec[where x=R]]
+        by (meson INTERP_SPEC prems(4) set_mult_expn)
+      note this[simplified]
+      then show ?thesis
+        by (simp add: INTERP_SPEC set_mult_expn)
+    qed
+     apply (smt (z3) INTERP_SPEC LooseStateSpec_expn(2) LooseStateSpec_expn(3) set_mult_expn)
+    by blast .
+
+definition "Union_the_Same_Or_Arbitrary_when_Var Z X Y \<longleftrightarrow> (\<forall>v. (Z::'v \<Rightarrow> 'a set) v = X v + Y v)"
+
+lemma Union_the_Same_Or_Arbitrary_when_Var__the_Same:
+  \<open>Union_the_Same_Or_Arbitrary_when_Var Z Z Z\<close>
+  unfolding Union_the_Same_Or_Arbitrary_when_Var_def by simp
+
+lemma Union_the_Same_Or_Arbitrary_when_Var__Arbitrary:
+  \<open>Union_the_Same_Or_Arbitrary_when_Var (\<lambda>v. X v + Y v) X Y\<close>
+  unfolding Union_the_Same_Or_Arbitrary_when_Var_def by blast
+
+\<phi>reasoner_ML Union_the_Same_Or_Arbitrary_when_Var 1200
+  (\<open>Union_the_Same_Or_Arbitrary_when_Var ?Z ?X ?Y\<close>) = \<open>
+fn (ctxt,sequent) =>
+  let
+    val \<^const>\<open>Trueprop\<close> $ (Const (\<^const_name>\<open>Union_the_Same_Or_Arbitrary_when_Var\<close>, _)
+          $ Z $ _ $ _) = Thm.major_prem_of sequent
+  in (ctxt,
+        (if is_Var (Envir.beta_eta_contract Z)
+         then @{thm Union_the_Same_Or_Arbitrary_when_Var__Arbitrary}
+         else @{thm Union_the_Same_Or_Arbitrary_when_Var__the_Same})
+        RS sequent) |> Seq.single
+  end
+\<close>
+
+proc (nodef) try'':
+  assumes F: \<open>\<p>\<r>\<o>\<c> f \<lbrace> X \<longmapsto> YY \<rbrace> \<t>\<h>\<r>\<o>\<w>\<s> E \<close>
+  assumes G: \<open>(\<And>v. \<p>\<r>\<o>\<c> g v \<lbrace> E v \<longmapsto> YY \<rbrace> \<t>\<h>\<r>\<o>\<w>\<s> EE2 )\<close>
+  input  X
+    output YY
+  throws EE2
+  \<medium_left_bracket> "__op_try__"
+    F
+    G
+  \<medium_right_bracket> .
+
+proc (nodef) try':
+  assumes A: \<open>Union_the_Same_Or_Arbitrary_when_Var Z Y1 Y2\<close>
+  assumes F: \<open>\<p>\<r>\<o>\<c> f \<lbrace> X \<longmapsto> Y1 \<rbrace> \<t>\<h>\<r>\<o>\<w>\<s> E \<close>
+  assumes G: \<open>\<And>v. \<p>\<r>\<o>\<c> g v \<lbrace> E v \<longmapsto> Y2 \<rbrace> \<t>\<h>\<r>\<o>\<w>\<s> E2 \<close>
+  input  X
+    output Z
+  throws E2
+  \<medium_left_bracket> "__op_try__" F G
+    unfold A[unfolded Union_the_Same_Or_Arbitrary_when_Var_def, THEN spec, symmetric]
+  \<medium_right_bracket>.
+
+
+
+
+
+end
