Phi_System/Resource_Template.thy
@@ -1,0 +1,957 @@
+theory Resource_Template
+  imports PhiSem_Formalization_Tools2 Phi_Semantics_Framework.Phi_SemFrame_ex
+begin
+
+
+chapter \<open>Resource Bases and Templates\<close>
+
+section \<open>Preliminary\<close>
+
+interpretation to_share: cancl_perm_ins_homo \<open>to_share::'a::nonsepable_semigroup option \<Rightarrow> 'a share option\<close> ..
+interpretation pointwise_to_share:
+  cancl_perm_ins_homo \<open>(o) (to_share::'a::nonsepable_semigroup option \<Rightarrow> 'a share option)\<close> ..
+
+section \<open>Bases\<close>
+
+subsection \<open>Resource Base\<close>
+
+locale resource =
+  resource_kind RES.DOMAIN Res
+  for Res :: "'T::sep_algebra resource_entry"
+begin
+
+lemma get_res_valid_raw: (*TODO: depreciated?*)
+  \<open> res \<in> RES.SPACE
+\<Longrightarrow> get res \<in>\<^sub>S\<^sub>H domain\<close>
+  unfolding RES.SPACE_def
+  by (simp, metis in_DOMAIN proj_inj)
+
+definition \<open>basic_fiction = Interp (\<lambda>x. { 1(Res #= x) })\<close>
+
+lemma basic_fiction_\<I>:
+  "\<I> basic_fiction = (\<lambda>x. { 1(Res #= x)})"
+  unfolding basic_fiction_def
+  by (rule Interp_inverse) (clarsimp simp add: Interpretation_def one_set_def)
+
+subsubsection \<open>Getter\<close>
+
+definition \<phi>R_get_res' :: \<open>'T proc\<close> \<comment> \<open>use this\<close>
+  where \<open>\<phi>R_get_res' = (\<lambda>res. Return (\<phi>arg (get res)) res)\<close>
+
+lemma \<phi>R_get_res'_valid:
+  \<open>Valid_Proc \<phi>R_get_res'\<close>
+  unfolding Valid_Proc_def \<phi>R_get_res'_def Return_def det_lift_def
+  by simp
+
+lemma \<phi>R_get_res_transition:
+  \<open> Transition_of' \<phi>R_get_res' ret = Id_on {s. s \<in> SPACE \<and> ret = Normal (\<phi>arg (get s))}\<close>
+  unfolding Transition_of'_def \<phi>R_get_res'_def Return_def det_lift_def
+  by (cases ret; clarsimp simp add: set_eq_iff Id_on_iff; blast)
+
+subsubsection \<open>Setter\<close>
+
+definition \<phi>R_set_res' :: \<open>('T \<Rightarrow> 'T) \<Rightarrow> unit proc\<close>
+  where \<open>\<phi>R_set_res' F = (\<lambda>res. if updt F res \<in> SPACE
+                                then {Success (\<phi>arg ()) (updt F res)}
+                                else {Invalid})\<close>
+
+lemma setter_transition:
+  \<open> (\<forall>m. m \<in>\<^sub>S\<^sub>H domain \<longrightarrow> P m \<longrightarrow> F m \<in>\<^sub>S\<^sub>H domain)
+\<Longrightarrow> Transition_of' (\<phi>R_set_res' F) ret
+ \<subseteq> {(x,y). x \<in> SPACE \<and> (P (get x) \<longrightarrow> y = updt F x \<and> ret = Normal \<phi>V_none)}\<close>
+  unfolding Transition_of'_def \<phi>R_set_res'_def
+  apply (cases ret; auto simp add: set_eq_iff \<phi>V_none_def if_split_mem2)
+  by (metis \<r>_valid_split fun_upd_same fun_upd_upd proj_inj)
+
+lemma setter_valid:
+  \<open>Valid_Proc (\<phi>R_set_res' F)\<close>
+  unfolding Valid_Proc_def \<phi>R_set_res'_def bind_def Return_def det_lift_def
+  by (clarsimp split: option.split)
+
+
+
+end
+
+
+subsection \<open>Fiction Base\<close>
+
+locale basic_fiction =
+   R: resource Res
++  fiction_kind FIC.DOMAIN INTERPRET Fic \<open>R.basic_fiction \<circ>\<^sub>\<I> I\<close>
+for Res :: "'T::sep_algebra resource_entry"
+and I :: "('U::sep_algebra, 'T) interp"
+and Fic :: "'U fiction_entry"
+begin
+
+subsubsection \<open>\<phi>-Type\<close>
+
+definition \<phi> :: \<open>('U, 'x) \<phi> \<Rightarrow> (fiction, 'x) \<phi>\<close>
+    \<comment> \<open>\<phi>Type for level-1 mapping\<close>
+  where \<open>\<phi> T = (\<lambda>x. { mk v |v. v \<in> (x \<Ztypecolon> T) })\<close>
+
+lemma \<phi>_expn[\<phi>expns]:
+  \<open>p \<in> (x \<Ztypecolon> \<phi> T) \<longleftrightarrow> (\<exists>v. p = mk v \<and> v \<in> (x \<Ztypecolon> T))\<close>
+  unfolding \<phi>Type_def \<phi>_def by simp
+
+lemma \<phi>_inhabited[\<phi>inhabitance_rule, elim!]:
+  \<open>Inhabited (x \<Ztypecolon> \<phi> T) \<Longrightarrow> (Inhabited (x \<Ztypecolon> T) \<Longrightarrow> C) \<Longrightarrow> C\<close>
+  unfolding Inhabited_def by (simp add: \<phi>expns)
+
+lemma \<phi>_Prod:
+  \<open> \<phi> T \<^emph> \<phi> U = \<phi> (T \<^emph> U)\<close>
+  apply (rule \<phi>Type_eqI; clarsimp simp add: \<phi>expns; rule; clarsimp)
+  apply (metis mk_homo_mult)
+  by (metis fun_1upd_homo inj.homo_mult sep_disj_mk)
+
+lemma \<phi>_\<phi>None:
+  \<open>\<phi> \<circle> = \<circle>\<close>
+  by (rule \<phi>Type_eqI; simp add: \<phi>expns)
+
+lemma \<phi>_unit:
+  \<open>(1 \<Ztypecolon> \<phi> Identity) = Void\<close>
+  by (clarsimp simp add: set_eq_iff \<phi>_expn Identity_expn)
+
+lemma [\<phi>reason 1200 for \<open>(?x \<Ztypecolon> \<phi> \<circle>) = ?Z @action clean_automation_waste\<close>]:
+  \<open>(x \<Ztypecolon> \<phi> \<circle>) = (() \<Ztypecolon> \<circle>) @action clean_automation_waste\<close>
+  unfolding Action_Tag_def \<phi>_\<phi>None by simp
+
+lemma [\<phi>reason 1300 for \<open>(?x \<Ztypecolon> \<phi> \<circle>) = ?Z @action clean_automation_waste\<close>]:
+  \<open>(x \<Ztypecolon> \<phi> \<circle>) = 1 @action clean_automation_waste\<close>
+  unfolding Action_Tag_def \<phi>_\<phi>None by simp
+
+
+(*
+lemma [\<phi>reason 1500 for \<open>(x \<Ztypecolon> \<phi> \<circle>) \<i>\<m>\<p>\<l>\<i>\<e>\<s> ?Y \<a>\<n>\<d> ?P @action (?Act::?'act::simplification action)\<close>]:
+  \<open>(x \<Ztypecolon> \<phi> \<circle>) \<i>\<m>\<p>\<l>\<i>\<e>\<s> (() \<Ztypecolon> \<circle>) @action Act\<close>
+  for Act :: \<open>'act::simplification action\<close>
+  unfolding Action_Tag_def \<phi>_\<phi>None
+  by (simp add: implies_refl) *)
+
+paragraph \<open>Reasoning Rules\<close>
+
+lemma \<phi>_cast:
+  \<open> x \<Ztypecolon> T \<i>\<m>\<p>\<l>\<i>\<e>\<s> y \<Ztypecolon> U \<a>\<n>\<d> P
+\<Longrightarrow> x \<Ztypecolon> \<phi> T \<i>\<m>\<p>\<l>\<i>\<e>\<s> y \<Ztypecolon> \<phi> U \<a>\<n>\<d> P\<close>
+  unfolding Imply_def by (clarsimp simp add: \<phi>expns)
+
+lemma \<phi>_Structural_Extract:
+  \<open> Structural_Extract (x \<Ztypecolon> T) (r \<Ztypecolon> R) (y \<Ztypecolon> U) (w \<Ztypecolon> W) P
+\<Longrightarrow> Structural_Extract (x \<Ztypecolon> \<phi> T) (r \<Ztypecolon> \<phi> R) (y \<Ztypecolon> \<phi> U) (w \<Ztypecolon> \<phi> W) P\<close>
+  unfolding Structural_Extract_def
+  by (simp add: \<phi>Prod_expn'[symmetric] \<phi>_Prod \<phi>_cast)
+
+declare \<phi>_Structural_Extract[THEN SE_clean_waste, \<phi>reason 1200]
+
+lemma [THEN SE_clean_waste', \<phi>reason 1211]:
+  \<open> Structural_Extract (x \<Ztypecolon> T) (r \<Ztypecolon> R) (y \<Ztypecolon> U) (w \<Ztypecolon> W)
+      (Automatic_Morphism RP (Structural_Extract (y' \<Ztypecolon> U') (w' \<Ztypecolon> W') (x' \<Ztypecolon> T') (r' \<Ztypecolon> R') P') \<and> P)
+\<Longrightarrow> Structural_Extract (x \<Ztypecolon> \<phi> T) (r \<Ztypecolon> \<phi> R) (y \<Ztypecolon> \<phi> U) (w \<Ztypecolon> \<phi> W)
+      (Automatic_Morphism RP (Structural_Extract (y' \<Ztypecolon> \<phi> U') (w' \<Ztypecolon> \<phi> W') (x' \<Ztypecolon> \<phi> T') (r' \<Ztypecolon> \<phi> R') P') \<and> P)\<close>
+  unfolding Automatic_Transformation_def Action_Tag_def
+  by (blast intro: \<phi>_Structural_Extract[unfolded Action_Tag_def]
+                   Structural_Extract_imply_P)
+
+lemma ToSA_by_structural_extraction:
+  " Structure_Info U Q
+\<Longrightarrow> \<s>\<i>\<m>\<p>\<l>\<i>\<f>\<y> Q' : Q
+\<Longrightarrow> (Q' \<Longrightarrow> \<r>CALL Try Any (Structural_Extract (y \<Ztypecolon> \<phi> U) R1 (x \<Ztypecolon> \<phi> T) W P2))
+\<Longrightarrow> A \<i>\<m>\<p>\<l>\<i>\<e>\<s> R2 \<heavy_comma> \<blangle> W \<brangle> \<a>\<n>\<d> P1
+\<Longrightarrow> A \<heavy_comma> y \<Ztypecolon> \<phi> U \<i>\<m>\<p>\<l>\<i>\<e>\<s> R2\<heavy_comma> R1\<heavy_comma> \<blangle> x \<Ztypecolon> \<phi> T \<brangle> \<a>\<n>\<d> P1 \<and> P2"
+  unfolding Premise_def FOCUS_TAG_def Structural_Extract_def Simplify_def Try_def \<r>Call_def
+  \<medium_left_bracket> premises SI and Q and SE and A
+  have \<open>Q'\<close> using \<phi> SI[unfolded Structure_Info_def] Q by blast
+  ;;  A[THEN implies_right_prod]
+     SE[OF \<open>Q'\<close>]
+  \<medium_right_bracket> certified using \<phi> by simp .
+
+lemma ToSA_by_structural_extraction__reverse_morphism:
+  " Structure_Info U Q
+\<Longrightarrow> \<s>\<i>\<m>\<p>\<l>\<i>\<f>\<y> Q' : Q
+\<Longrightarrow> (Q' \<Longrightarrow> \<r>CALL Try Any (Structural_Extract (y \<Ztypecolon> \<phi> U) R1 (x \<Ztypecolon> \<phi> T) W
+             (Automatic_Morphism RP2 (Structural_Extract (x' \<Ztypecolon> \<phi> T') W' (y' \<Ztypecolon> \<phi> U') R1' P2') \<and> P2)))
+\<Longrightarrow> A \<i>\<m>\<p>\<l>\<i>\<e>\<s> R2 \<heavy_comma> \<blangle> W \<brangle> \<a>\<n>\<d> (Automatic_Morphism RP1 (R2'\<heavy_comma> \<blangle> W' \<brangle> \<i>\<m>\<p>\<l>\<i>\<e>\<s> A' \<a>\<n>\<d> P1') \<and> P1)
+\<Longrightarrow> A \<heavy_comma> y \<Ztypecolon> \<phi> U \<i>\<m>\<p>\<l>\<i>\<e>\<s> R2\<heavy_comma> R1\<heavy_comma> \<blangle> x \<Ztypecolon> \<phi> T \<brangle> \<a>\<n>\<d>
+      (Automatic_Morphism (RP2 \<and>\<^sub>\<r> RP1) (R2'\<heavy_comma> R1'\<heavy_comma> \<blangle> x' \<Ztypecolon> \<phi> T' \<brangle> \<i>\<m>\<p>\<l>\<i>\<e>\<s> A'\<heavy_comma> y' \<Ztypecolon> \<phi> U' \<a>\<n>\<d> P1' \<and> P2')
+          \<and> P1 \<and> P2)"
+  unfolding Premise_def FOCUS_TAG_def Structural_Extract_def Simplify_def
+            Automatic_Transformation_def Compact_Antecedent_def Try_def \<r>Call_def
+  \<medium_left_bracket> premises SI and Q and SE and A
+  have \<open>Q'\<close> using \<phi> SI[unfolded Structure_Info_def] Q by blast
+  ;; A[THEN implies_right_prod]
+     SE[OF \<open>Q'\<close>]
+  \<medium_right_bracket> certified apply  (simp add: \<phi>)
+  \<medium_left_bracket>
+    have A : \<open>R2' \<heavy_comma> W' \<i>\<m>\<p>\<l>\<i>\<e>\<s> A' \<a>\<n>\<d> P1'\<close> using \<phi>_previous \<open>RP2 \<and> RP1\<close> by simp
+    have SE: \<open>(R1' \<heavy_comma> x' \<Ztypecolon> \<phi> T' \<i>\<m>\<p>\<l>\<i>\<e>\<s> W' \<heavy_comma> y' \<Ztypecolon> \<phi> U' \<a>\<n>\<d> P2')\<close> using \<phi>_previous \<open>RP2 \<and> RP1\<close> by simp
+    ;; SE A[THEN implies_right_prod]
+  \<medium_right_bracket>. .
+
+
+lemma ToSA_skip [\<phi>reason 1200 except \<open> _ \<heavy_comma> ?y \<Ztypecolon> \<phi> ?U \<i>\<m>\<p>\<l>\<i>\<e>\<s> _ \<heavy_comma> \<blangle> ?x \<Ztypecolon> \<phi> ?T \<brangle> \<a>\<n>\<d> _\<close> ]:
+  " R \<i>\<m>\<p>\<l>\<i>\<e>\<s> R'\<heavy_comma> \<blangle> x \<Ztypecolon> \<phi> T \<brangle> \<a>\<n>\<d> P
+\<Longrightarrow> R \<heavy_comma> X \<i>\<m>\<p>\<l>\<i>\<e>\<s> R'\<heavy_comma> X\<heavy_comma> \<blangle> x \<Ztypecolon> \<phi> T \<brangle> \<a>\<n>\<d> P"
+  unfolding Action_Tag_def FOCUS_TAG_def split_paired_All Action_Tag_def
+  by (metis ab_semigroup_mult_class.mult_ac(1) implies_left_prod mult.commute)
+
+lemma [\<phi>reason 1200]:
+  \<open> x \<Ztypecolon> T \<i>\<m>\<p>\<l>\<i>\<e>\<s> y \<Ztypecolon> U \<a>\<n>\<d> P @action \<A>_structural Act
+\<Longrightarrow> x \<Ztypecolon> \<phi> T \<i>\<m>\<p>\<l>\<i>\<e>\<s> y \<Ztypecolon> \<phi> U \<a>\<n>\<d> P @action \<A>_structural Act \<close>
+  unfolding Action_Tag_def using \<phi>_cast .
+
+lemma [\<phi>reason 1200]:
+  \<open> x \<Ztypecolon> T \<i>\<m>\<p>\<l>\<i>\<e>\<s> y \<Ztypecolon> U \<a>\<n>\<d> P @action to Target
+\<Longrightarrow> x \<Ztypecolon> \<phi> T \<i>\<m>\<p>\<l>\<i>\<e>\<s> y \<Ztypecolon> \<phi> U \<a>\<n>\<d> P @action to Target \<close>
+  unfolding Action_Tag_def using \<phi>_cast .
+
+
+lemma [\<phi>reason 1200]:
+  \<open> \<r>Clean (x \<Ztypecolon> T)
+\<Longrightarrow> \<r>Clean (x \<Ztypecolon> \<phi> T) \<close>
+  unfolding \<r>Clean_def Imply_def apply (simp add: \<phi>expns)
+  using mk_homo_one by blast
+
+lemma [\<phi>reason 1200 for \<open>If _ (_ \<Ztypecolon> \<phi> _) (_ \<Ztypecolon> \<phi> _) \<i>\<m>\<p>\<l>\<i>\<e>\<s> _ @action branch_convergence\<close>]:
+  \<open> If P (x \<Ztypecolon> T) (y \<Ztypecolon> U) \<i>\<m>\<p>\<l>\<i>\<e>\<s> (z \<Ztypecolon> Z) @action branch_convergence
+\<Longrightarrow> If P (x \<Ztypecolon> \<phi> T) (y \<Ztypecolon> \<phi> U) \<i>\<m>\<p>\<l>\<i>\<e>\<s> (z \<Ztypecolon> \<phi> Z) @action branch_convergence\<close>
+  unfolding Action_Tag_def by (cases P; simp add: \<phi>_cast)
+
+paragraph \<open>Conversion\<close>
+
+lemma [simp]:
+  \<open>(\<phi> (ExTyp T)) = (\<exists>\<phi> c. \<phi> (T c))\<close>
+  by (rule \<phi>Type_eqI; clarsimp simp add: \<phi>expns; blast)
+
+lemma [simp]:
+  \<open>(\<phi> (T \<phi>\<s>\<u>\<b>\<j> P)) = (\<phi> T \<phi>\<s>\<u>\<b>\<j> P)\<close>
+  by (rule \<phi>Type_eqI; clarsimp simp add: \<phi>expns; blast)
+
+lemma \<phi>_simp_cong[folded atomize_eq]:
+  \<open> (x \<Ztypecolon> T) = (x' \<Ztypecolon> T')
+\<Longrightarrow> (x \<Ztypecolon> \<phi> T) = (x' \<Ztypecolon> \<phi> T')\<close>
+  unfolding set_eq_iff by (simp add: \<phi>expns)
+
+simproc_setup \<phi>\<phi>_simp_cong ("x \<Ztypecolon> \<phi> T") = \<open>
+  K (fn ctxt => Phi_SimpCong.simproc @{thm \<phi>_simp_cong} ctxt)
+\<close>
+
+paragraph \<open>Synthesis for moving\<close>
+
+lemma [\<phi>reason 1200 for
+  \<open>Synthesis_Parse (\<phi> ?T) (?Y::?'ret \<Rightarrow> assn)\<close>
+]:
+  \<open>Synthesis_Parse (\<phi> T) (\<lambda>_. x \<Ztypecolon> \<phi> T :: assn)\<close>
+  unfolding Synthesis_Parse_def ..
+
+(* lemma [\<phi>reason for \<open>\<p>\<r>\<o>\<c> ?f \<lbrace> ?S1 \<longmapsto> \<lambda>ret. ?S2\<heavy_comma>  \<blangle> ?x \<Ztypecolon> \<phi> ?T \<brangle> \<rbrace> \<t>\<h>\<r>\<o>\<w>\<s> ?E\<close>]:
+  \<open> SUBGOAL G G'
+\<Longrightarrow> S1 \<i>\<m>\<p>\<l>\<i>\<e>\<s> S2\<heavy_comma> \<blangle> x \<Ztypecolon> \<phi> T \<brangle>
+\<Longrightarrow> SOLVE_SUBGOAL G'
+\<Longrightarrow> \<p>\<r>\<o>\<c> Return \<phi>V_none \<lbrace> S1 \<longmapsto> \<lambda>_. S2\<heavy_comma> \<blangle> x \<Ztypecolon> \<phi> T \<brangle> \<rbrace>\<close>
+  unfolding FOCUS_TAG_def Synthesis_def Action_Tag_def
+  using \<phi>__Return_rule__ view_shift_by_implication by blast *)
+
+
+subsubsection \<open>Fictional Refinement\<close>
+
+context begin
+
+private lemma from_fictional_refinement':
+  \<open> Valid_Proc f
+\<Longrightarrow> (\<And>v. Transition_of' f v \<r>\<e>\<f>\<i>\<n>\<e>\<s> Rel v \<w>.\<r>.\<t> R.basic_fiction o\<^sub>\<I> I \<i>\<n> D)
+\<Longrightarrow> Valid_Transition Rel
+\<Longrightarrow> x \<in> D
+\<Longrightarrow> \<p>\<r>\<o>\<c> f \<lbrace> x \<Ztypecolon> \<phi> Identity \<longmapsto> \<lambda>v. y \<Ztypecolon> \<phi> Identity \<s>\<u>\<b>\<j> y. (x,y) \<in> Rel (Normal v) \<rbrace> \<t>\<h>\<r>\<o>\<w>\<s> (\<lambda>e. y \<Ztypecolon> \<phi> Identity \<s>\<u>\<b>\<j> y. (x,y) \<in> Rel (Abnm e))\<close>
+  unfolding \<phi>Procedure_alt Fictional_Forward_Simulation_def atomize_all Valid_Transition_def
+  apply (auto simp add: Image_iff subset_iff Bex_def R.basic_fiction_\<I> \<phi>expns Transition_of'_def
+          LooseStateSpec_def split_sum_all INTERP_RES_def interp_split' R.\<r>_valid_split' interp_comp_\<I>
+          R.inject_wand_homo inject_wand_homo prj.homo_mult eval_stat_forall split: eval_stat.split)
+  subgoal premises prems for r u y v y' rr
+    thm prems
+    thm prems(4)[THEN spec[where x=v], THEN spec[where x=x], THEN spec[where x=\<open>get r\<close>], THEN spec[where x=\<open>{u}\<close>], THEN spec[where x=\<open>y'\<close>]]
+  proof -
+    have t2: \<open>(\<exists>xa. (\<exists>ua v. xa = ua * v \<and> ua \<in> {u} \<and> (\<exists>xa. xa \<in> \<I> I (get r * x) \<and> v = R.mk xa) \<and> ua ## v) \<and>
+      get r ## x \<and> x \<in> D \<and> Success v y' \<in> f xa \<and> R.clean xa \<in> R.SPACE \<and> (\<exists>m. xa R.name = R.inject m \<and> m \<in>\<^sub>S\<^sub>H R.domain))\<close>
+      apply (rule exI[where x=\<open>(u * R.mk y)\<close>], simp add: prems R.inj.homo_mult[symmetric] )
+      using prems(11) prems(12) by blast
+    note prems(4)[THEN spec[where x=v], THEN spec[where x=x], THEN spec[where x=\<open>get r\<close>], THEN spec[where x=\<open>{u}\<close>], THEN spec[where x=\<open>y'\<close>],
+            THEN mp, OF this]
+    then show ?thesis
+    apply clarsimp
+    subgoal for yy ya
+      apply (rule exI[where x=yy], clarsimp simp add: inj.homo_mult[symmetric] prems prj.homo_mult, rule)
+      apply (metis R.resource_kind_axioms Valid_Proc_def prems(1) prems(14) resource_kind.\<r>_valid_split t2 times_fupdt_1_apply_sep)
+      using prems(10) by blast .
+qed
+  subgoal premises prems for r u y v y' rr
+  proof -
+    thm prems(5)[THEN spec[where x=v], THEN spec[where x=x], THEN spec[where x=\<open>get r\<close>], THEN spec[where x=\<open>{u}\<close>], THEN spec[where x=\<open>y'\<close>]]
+    have t2: \<open>(\<exists>xa. (\<exists>ua v. xa = ua * v \<and> ua \<in> {u} \<and> (\<exists>xa. xa \<in> \<I> I (get r * x) \<and> v = R.mk xa) \<and> ua ## v) \<and>
+      get r ## x \<and> x \<in> D \<and> Abnormal v y' \<in> f xa \<and> R.clean xa \<in> R.SPACE \<and> (\<exists>m. xa R.name = R.inject m \<and> m \<in>\<^sub>S\<^sub>H R.domain))\<close>
+      by (metis (no_types, lifting) R.inj.homo_mult fiction_kind.sep_disj_get_name_eq fiction_kind_axioms insert_iff mult_in_sep_homo_set prems(11) prems(12) prems(13) prems(14) prems(15) prems(16) prems(17) prems(3) prems(7) prems(8) prems(9) times_fupdt_1_apply_sep times_fupdt_1_fupdt_1_sep)
+    note prems(5)[THEN spec[where x=v], THEN spec[where x=x], THEN spec[where x=\<open>get r\<close>], THEN spec[where x=\<open>{u}\<close>], THEN spec[where x=\<open>y'\<close>],
+            THEN mp, OF this]
+    then show ?thesis
+      apply clarsimp
+      subgoal for yy ya
+        apply (rule exI[where x=yy], clarsimp simp add: inj.homo_mult[symmetric] prems prj.homo_mult, rule)
+        apply (metis R.\<r>_valid_split Valid_Proc_def prems(1) prems(14) t2 times_fupdt_1_apply_sep)
+        using prems(10) by blast .
+  qed
+  by (metis (no_types, lifting) R.inj.homo_mult mult_in_sep_homo_set sep_disj_get_name times_fupdt_1_apply_sep times_fupdt_1_fupdt_1_sep)
+
+
+lemma from_fictional_refinement:
+  \<open> Valid_Proc f
+\<Longrightarrow> YY = (\<lambda>v. y \<Ztypecolon> \<phi> Identity \<s>\<u>\<b>\<j> y. (x,y) \<in> Rel (Normal v))
+\<Longrightarrow> EE = (\<lambda>e. y \<Ztypecolon> \<phi> Identity \<s>\<u>\<b>\<j> y. (x,y) \<in> Rel (Abnm e))
+\<Longrightarrow> (\<And>v. Transition_of' f v \<r>\<e>\<f>\<i>\<n>\<e>\<s> Rel v \<w>.\<r>.\<t> R.basic_fiction o\<^sub>\<I> I \<i>\<n> D)
+\<Longrightarrow> Valid_Transition Rel
+\<Longrightarrow> x \<in> D
+\<Longrightarrow> \<p>\<r>\<o>\<c> f \<lbrace> x \<Ztypecolon> \<phi> Identity \<longmapsto> YY \<rbrace> \<t>\<h>\<r>\<o>\<w>\<s> EE\<close>
+  using from_fictional_refinement' by blast
+
+end
+
+lemma "__getter_rule__":
+  \<open> Valid_Proc getter
+\<Longrightarrow> (\<And>ret. Transition_of' getter ret \<r>\<e>\<f>\<i>\<n>\<e>\<s> Id_on ({x} \<s>\<u>\<b>\<j> ret = Normal (\<phi>arg v)) \<w>.\<r>.\<t> R.basic_fiction o\<^sub>\<I> I \<i>\<n> {x})
+\<Longrightarrow> \<p>\<r>\<o>\<c> getter \<lbrace> x \<Ztypecolon> \<phi> Identity \<longmapsto> \<lambda>ret. x \<Ztypecolon> \<phi> Identity \<s>\<u>\<b>\<j> ret = \<phi>arg v \<rbrace>\<close>
+  by (rule from_fictional_refinement[where Rel = \<open>\<lambda>ret. Id_on ({x} \<s>\<u>\<b>\<j> ret = Normal (\<phi>arg v))\<close>
+                                       and D = \<open>{x}\<close>],
+     assumption,
+     clarsimp simp add: set_eq_iff Subjection_expn Id_on_iff ExSet_expn,
+     simp add: Id_on_iff zero_set_def zero_fun_def,
+     assumption,
+     simp add: Valid_Transition_def zero_set_def,
+     simp)
+
+lemma "__setter_rule__":
+  \<open> Valid_Proc setter
+\<Longrightarrow> (\<And>ret. Transition_of' setter ret \<r>\<e>\<f>\<i>\<n>\<e>\<s> {(x,y)} \<s>\<u>\<b>\<j> ret = Normal \<phi>V_none
+            \<w>.\<r>.\<t> R.basic_fiction o\<^sub>\<I> I \<i>\<n> {x})
+\<Longrightarrow> \<p>\<r>\<o>\<c> setter \<lbrace> x \<Ztypecolon> \<phi> Identity \<longmapsto> \<lambda>_. y \<Ztypecolon> \<phi> Identity \<rbrace>\<close>
+  by (rule from_fictional_refinement
+                  [where Rel=\<open>\<lambda>ret. {(x,y)} \<s>\<u>\<b>\<j> ret = Normal \<phi>V_none\<close> and D = \<open>{x}\<close>],
+      assumption,
+      clarsimp simp add: set_eq_iff Subjection_expn Id_on_iff ExSet_expn \<phi>arg_All fun_eq_iff \<phi>V_none_def,
+      simp add: Id_on_iff zero_set_def zero_fun_def,
+      assumption,
+      simp add: Valid_Transition_def zero_set_def,
+      simp)
+
+lemma "__allocator_rule__":
+  \<open> Valid_Proc allocator
+\<Longrightarrow> (\<And>ret. Transition_of' allocator ret \<r>\<e>\<f>\<i>\<n>\<e>\<s> {(1,y k)} \<s>\<u>\<b>\<j> k. ret = Normal (\<phi>arg k) \<and> P k
+            \<w>.\<r>.\<t> R.basic_fiction o\<^sub>\<I> I \<i>\<n> {1})
+\<Longrightarrow> \<p>\<r>\<o>\<c> allocator \<lbrace> Void \<longmapsto> \<lambda>ret. y k \<Ztypecolon> \<phi> Identity \<s>\<u>\<b>\<j> k. ret = \<phi>arg k \<and> P k \<rbrace>\<close>
+  by (rule from_fictional_refinement
+        [where Rel=\<open>\<lambda>ret. {(1,y k)} \<s>\<u>\<b>\<j> k. ret = Normal (\<phi>arg k) \<and> P k\<close>
+           and x=\<open>1\<close> and D=\<open>{1}\<close>, unfolded \<phi>_unit],
+      assumption,
+      clarsimp simp add: set_eq_iff Subjection_expn Id_on_iff ExSet_expn \<phi>arg_All fun_eq_iff \<phi>V_none_def,
+      simp add: Id_on_iff zero_set_def zero_fun_def,
+      assumption,
+      simp add: Valid_Transition_def zero_set_def,
+      simp)
+
+end
+
+(*
+subsubsection \<open>Permission Fiction\<close>
+
+locale permission_fiction =
+   R: resource Res
++  share: perm_ins_homo \<psi>
++  fiction_kind FIC.DOMAIN INTERPRET Fic
+      \<open>R.basic_fiction \<circ>\<^sub>\<I> (\<F>_functional \<psi>)\<close>
+for Res :: "'T::sep_algebra resource_entry"
+and \<psi> :: \<open>'T \<Rightarrow> 'U::{share_sep_disj,share_module_sep,sep_algebra}\<close>
+and Fic :: "'U fiction_entry"
+begin
+
+sublocale basic_fiction Res \<open>\<F>_functional \<psi>\<close> ..
+
+
+paragraph \<open>Reasoning Rules\<close>
+
+declare ToSA_by_structural_extraction
+    [\<phi>reason 1210 if \<open>PLPR_Env.boolean_flag \<^const_name>\<open>ToA_flag_deep\<close> true o fst\<close>]
+declare ToSA_by_structural_extraction__reverse_morphism
+    [\<phi>reason 1213 if \<open>PLPR_Env.boolean_flag \<^const_name>\<open>ToA_flag_deep\<close> true o fst\<close>]
+
+end
+*)
+
+
+
+(*
+subsubsection \<open>Identity Fiction\<close>
+
+locale identity_fiction =
+   R: resource Res
++  fiction_kind FIC.DOMAIN INTERPRET Fic \<open>R.basic_fiction o\<^sub>\<I> \<F>_it\<close>
+for Res :: "'T::sep_algebra resource_entry"
+and Fic :: "'T fiction_entry"
+begin
+
+sublocale basic_fiction where I = \<open>\<F>_it\<close> ..
+
+declare ToSA_by_structural_extraction
+   [\<phi>reason 1210 if \<open>PLPR_Env.boolean_flag \<^const_name>\<open>ToA_flag_deep\<close> true o fst\<close>]
+declare ToSA_by_structural_extraction__reverse_morphism
+   [\<phi>reason 1213 if \<open>PLPR_Env.boolean_flag \<^const_name>\<open>ToA_flag_deep\<close> true o fst\<close>]
+
+end
+*)
+
+
+
+
+section \<open>Non-separable Monolithic Resource\<close>
+  \<comment> \<open>The resource non-sepable and having type shape \<^typ>\<open>'a::nonsepable_semigroup option\<close>\<close>
+
+locale nonsepable_mono_resource =
+  resource Res
+for Res :: "'T nosep option resource_entry"
+begin
+
+abbreviation fiction_agree
+  where \<open>fiction_agree \<equiv> basic_fiction o\<^sub>\<I> \<F>_optionwise \<F>_agree\<close>
+
+end
+
+
+subsubsection \<open>Interp Agreement\<close>
+
+(*TODO: ('k \<Rightarrow> 'v) nosep option ----> ('k \<Rightarrow> 'v share option)
+  total to that
+  none to none
+ *)
+
+(*TODO!*)
+locale agreement_fiction_for_nosepable_mono_resource =
+   R: nonsepable_mono_resource Res
++  fiction_kind FIC.DOMAIN INTERPRET Fic \<open>R.fiction_agree\<close>
+for Res :: "'T nosep option resource_entry"
+and Fic :: "'T nosep agree option fiction_entry"
+begin
+
+sublocale basic_fiction Res \<open>\<F>_optionwise \<F>_agree\<close> Fic
+  by (standard; simp add: raw_domain)
+
+lemma double:
+  \<open>{mk x |x. P x} \<i>\<m>\<p>\<l>\<i>\<e>\<s> {mk x |x. P x} * {mk x |x. P x}\<close>
+  unfolding Imply_def
+  apply (clarsimp simp add: \<phi>expns mk_homo_mult[symmetric])
+  subgoal for x'
+    apply (rule exI[where x=\<open>mk x'\<close>], rule exI[where x=\<open>mk x'\<close>])
+    by (cases x'; simp add: mk_homo_mult[symmetric]) .
+
+lemma contract:
+  \<open>{mk x |x. P x} * {mk x |x. P x} \<i>\<m>\<p>\<l>\<i>\<e>\<s> {mk x |x. P x} \<close>
+  unfolding Imply_def
+  apply (clarsimp simp add: \<phi>expns)
+  subgoal for x y by (cases x; cases y; simp add: mk_homo_mult[symmetric]) .
+
+paragraph \<open>\<phi>-Type\<close>
+
+abbreviation \<open>\<phi>_ag T \<equiv> \<phi> (Agreement (Nosep T))\<close>
+
+declare ToSA_by_structural_extraction
+    [\<phi>reason 1210 if \<open>PLPR_Env.boolean_flag \<^const_name>\<open>ToA_flag_deep\<close> true o fst\<close>]
+declare ToSA_by_structural_extraction__reverse_morphism
+    [\<phi>reason 1213 if \<open>PLPR_Env.boolean_flag \<^const_name>\<open>ToA_flag_deep\<close> true o fst\<close>]
+
+lemma \<phi>_double_\<phi>app:
+  \<open>x \<Ztypecolon> \<phi>_ag T \<i>\<m>\<p>\<l>\<i>\<e>\<s> x \<Ztypecolon> \<phi>_ag T \<heavy_comma> x \<Ztypecolon> \<phi>_ag T\<close>
+proof -
+  have \<open>\<exists>P. (x \<Ztypecolon> \<phi>_ag T) = {mk x |x. P x}\<close>
+    unfolding set_eq_iff apply (simp add: \<phi>expns)
+    apply (rule exI[where x=\<open>\<lambda>y. \<exists>v. y = Some (agree (nosep v)) \<and> v \<in> (x \<Ztypecolon> T)\<close>])
+    by blast
+  then obtain P where [simp]: \<open>(x \<Ztypecolon> \<phi>_ag T) = {mk x |x. P x}\<close> by blast
+  show ?thesis by (simp add: double)
+qed
+
+lemma \<phi>_contract_\<phi>app:
+  \<open>x \<Ztypecolon> \<phi>_ag T \<heavy_comma> x \<Ztypecolon> \<phi>_ag T \<i>\<m>\<p>\<l>\<i>\<e>\<s> x \<Ztypecolon> \<phi>_ag T\<close>
+proof -
+  have \<open>\<exists>P. (x \<Ztypecolon> \<phi>_ag T) = {mk x |x. P x}\<close>
+    unfolding set_eq_iff apply (simp add: \<phi>expns)
+    apply (rule exI[where x=\<open>\<lambda>y. \<exists>v. y = Some (agree (nosep v)) \<and> v \<in> (x \<Ztypecolon> T)\<close>])
+    by blast
+  then obtain P where [simp]: \<open>(x \<Ztypecolon> \<phi>_ag T) = {mk x |x. P x}\<close> by blast
+  show ?thesis by (simp add: contract)
+qed
+
+end
+
+
+
+section \<open>Mapping Resources\<close>
+
+text \<open>Resources based on mapping\<close>
+
+locale mapping_resource =
+  resource Res
+for Res :: "('key \<Rightarrow> 'val::sep_algebra) resource_entry"
+begin
+
+definition
+    \<phi>R_allocate_res_entry' :: \<open>('key \<Rightarrow> bool)
+                           \<Rightarrow> 'val
+                           \<Rightarrow> 'key proc\<close>
+  where \<open>\<phi>R_allocate_res_entry' P init =
+    \<phi>R_get_res' \<bind> (\<lambda>res.
+    let k = (@k. \<phi>arg.dest res k = 1 \<and> P k)
+     in \<phi>R_set_res' (\<lambda>f. f(k := init))
+        \<ggreater> Return (\<phi>arg k)
+)\<close>
+
+lemma allocator_transition:
+  \<open> (\<forall>r. r \<in>\<^sub>S\<^sub>H domain \<longrightarrow> (\<exists>k. k \<notin> dom1 r \<and> P k))
+\<Longrightarrow> \<forall>k. P k \<longrightarrow> 1(k := init) \<in>\<^sub>S\<^sub>H domain
+\<Longrightarrow> Transition_of' (\<phi>R_allocate_res_entry' P init) ret
+        \<subseteq> (Id_on SPACE * {(1, mk (1(k := init))) | k. ret = Normal (\<phi>arg k) \<and> P k})\<close>
+  unfolding Transition_of'_def \<phi>R_allocate_res_entry'_def \<phi>R_get_res'_def bind_def Return_def
+      det_lift_def \<phi>R_set_res'_def Let_def
+  apply (cases ret; clarsimp simp add: zero_set_def set_eq_iff set_mult_expn Subjection_expn Id_on_iff)
+  apply (case_tac x; clarsimp simp add: zero_set_def set_eq_iff set_mult_expn Subjection_expn Id_on_iff)
+  subgoal premises prems for r b x 
+  proof -
+    have t1: \<open>get r \<in>\<^sub>S\<^sub>H domain\<close>
+      by (simp add: get_res_valid_raw prems(4))
+    let ?kk = \<open>SOME k. get r k = 1 \<and> P k\<close>
+    have t2: \<open>\<exists>k. get r k = 1 \<and> P k\<close>
+      using dom1_def prems(1) t1 by fastforce
+    have t3[simp]: \<open>get r ?kk = 1 \<and> P ?kk\<close>
+      by (insert t2; clarify; rule someI[where P=\<open>\<lambda>k. get r k = 1 \<and> P k\<close>]; blast)
+    have t4 [simp]: \<open>(get r)(?kk := init) = get r * 1(?kk := init)\<close>
+      by (simp add: fun_eq_iff)
+    have t5[simp]: \<open>get r ## 1(?kk := init)\<close>
+      by (metis (mono_tags, lifting) fun_sep_disj_1_fupdt(2) fun_upd_triv sep_disj_commuteI sep_magma_1_left t3)
+    have t6[simp]: \<open>r(name := inject ((get r)(?kk := init))) \<in> SPACE\<close>
+      by (metis comp.simps(6) empty_iff insert_iff prems(5))
+    have t61[simp]: \<open>r(name := inject (get r * 1(?kk := init))) \<in> SPACE\<close>
+      using t6 by auto
+    have t7[simp]: \<open>b = r(name := inject ((get r)(?kk := init)))\<close>
+      using prems[simplified] t4 by presburger 
+    show ?thesis
+      by (simp add: fun_eq_iff inj.homo_mult prems,
+          metis (no_types, lifting) fun_sep_disj_1_fupdt(1) fun_upd_triv inj.sep_disj_homo_semi inj_prj_in_SPACE prems(4) t5)
+  qed
+  subgoal premises prems for r proof -
+    let ?kk = \<open>SOME k. get r k = 1 \<and> P k\<close>
+    have t1: \<open>get r \<in>\<^sub>S\<^sub>H domain\<close>
+      by (simp add: get_res_valid_raw prems(5))
+    have t2: \<open>\<exists>k. get r k = 1 \<and> P k\<close>
+      using dom1_def prems(1) t1 by fastforce
+    have t3[simp]: \<open>get r ?kk = 1 \<and> P ?kk\<close>
+      by (insert t2; clarify; rule someI[where P=\<open>\<lambda>k. get r k = 1 \<and> P k\<close>]; blast)
+    have t4 [simp]: \<open>(get r)(?kk := init) = get r * 1(?kk := init)\<close>
+      by (simp add: fun_eq_iff)
+    have t5[simp]: \<open>get r ## 1(?kk := init)\<close>
+      by (metis (mono_tags, lifting) fun_sep_disj_1_fupdt(2) fun_upd_triv sep_disj_commuteI sep_magma_1_left t3)
+    have t7: \<open>r(name := inject ((get r)(?kk := init))) \<in> SPACE\<close>
+      by (metis (no_types, lifting) \<r>_valid_split fun_upd_same fun_upd_upd mult_in_sep_homo_set prems(2) prems(5) t1 t3 t4 t5)
+    show ?thesis
+      using prems(4) t7 by blast
+   qed .
+
+lemma allocator_refinement:
+  \<open> \<forall>r. r \<in>\<^sub>S\<^sub>H domain \<longrightarrow> (\<exists>k. k \<notin> dom1 r \<and> P k)
+\<Longrightarrow> \<forall>k. P k \<longrightarrow> 1(k := init) \<in>\<^sub>S\<^sub>H domain
+\<Longrightarrow> Transition_of' (\<phi>R_allocate_res_entry' P init) ret
+   \<r>\<e>\<f>\<i>\<n>\<e>\<s> {(1, 1(k := init))} \<s>\<u>\<b>\<j> k. ret = Normal (\<phi>arg k) \<and> P k
+   \<w>.\<r>.\<t> basic_fiction \<i>\<n> {1}\<close>
+  apply (rule refinement_sub_fun[OF allocator_transition], assumption, assumption)
+  unfolding Fictional_Forward_Simulation_def
+  apply (cases ret; clarsimp simp add: set_mult_expn Subjection_expn basic_fiction_\<I>
+      mk_homo_mult)
+  subgoal premises prems for r R u k
+  proof -
+    have [simp]: \<open>r ## 1(k := init)\<close>
+      using prems(5) prems(7) sep_disj_multD2 by blast
+    show ?thesis
+      apply (simp add: mk_homo_mult)
+      using prems(4) prems(5) prems(7) sep_disj_multI2 sep_mult_assoc by blast
+  qed .
+
+lemma allocator_valid:
+  \<open> \<forall>r. r \<in>\<^sub>S\<^sub>H domain \<longrightarrow> (\<exists>k. k \<notin> dom1 r \<and> P k)
+\<Longrightarrow> \<forall>k. P k \<longrightarrow> 1(k := init) \<in>\<^sub>S\<^sub>H domain
+\<Longrightarrow> Valid_Proc (\<phi>R_allocate_res_entry' P init)\<close>
+  unfolding Valid_Proc_def \<phi>R_allocate_res_entry'_def \<phi>R_get_res'_def \<phi>R_set_res'_def
+            bind_def Return_def det_lift_def Let_def
+  by (clarsimp split: option.split)
+
+end
+
+locale fiction_base_for_mapping_resource =
+  R: mapping_resource Res
++ fiction_kind FIC.DOMAIN INTERPRET Fic \<open>R.basic_fiction o\<^sub>\<I> I\<close>
+for Res :: "('key \<Rightarrow> 'val::sep_algebra) resource_entry"
+and I   :: "('T::sep_algebra, 'key \<Rightarrow> 'val) interp"
+and Fic :: "'T fiction_entry"
+begin
+
+sublocale basic_fiction Res I Fic ..
+
+lemma "__allocate_rule_2__":
+  \<open> (\<And>k. Id_on UNIV * {(1, 1(k := u))} \<r>\<e>\<f>\<i>\<n>\<e>\<s> {(1, u' k)} \<w>.\<r>.\<t> I \<i>\<n> {1})
+\<Longrightarrow> \<forall>k. P k \<longrightarrow> 1(k := u) \<in>\<^sub>S\<^sub>H R.domain
+\<Longrightarrow> \<forall>r. r \<in>\<^sub>S\<^sub>H R.domain \<longrightarrow> (\<exists>k. k \<notin> dom1 r \<and> P k)
+\<Longrightarrow> \<p>\<r>\<o>\<c> R.\<phi>R_allocate_res_entry' P u \<lbrace> Void \<longmapsto> \<lambda>ret. u' k \<Ztypecolon> \<phi> Identity \<s>\<u>\<b>\<j> k. ret = \<phi>arg k \<and> P k \<rbrace> \<close>
+  by (rule "__allocator_rule__",
+      rule R.allocator_valid,
+      assumption,
+      assumption,
+      rule sep_refinement_stepwise[
+        OF R.allocator_refinement[THEN refinement_frame[where R=UNIV]]],
+      assumption,
+      assumption,
+      unfold ExSet_times_right Subjection_times,
+      rule refinement_ExSet,
+      rule refinement_subjection,
+      assumption,
+      auto simp add: set_mult_expn)
+
+end
+
+
+section \<open>One Level Parital Mapping\<close>
+
+subsection \<open>Resource\<close>
+
+locale partial_map_resource =
+  mapping_resource Res
+for Res :: "('key \<Rightarrow> 'val::nonsepable_semigroup option) resource_entry"
+begin
+
+
+subsubsection \<open>Getter\<close>
+
+definition \<phi>R_get_res_entry' :: \<open>'key \<Rightarrow> 'val proc\<close>
+  where \<open>\<phi>R_get_res_entry' k =
+    \<phi>R_get_res' \<bind> (\<lambda>res. case \<phi>arg.dest res k of Some v \<Rightarrow> Return (\<phi>arg v) | _ \<Rightarrow> (\<lambda>_. {Invalid}))\<close>
+
+lemma getter_transition:
+  \<open> Transition_of' (\<phi>R_get_res_entry' k) ret
+        = Id_on {s. s \<in> SPACE \<and> ret = (case get s k of Some v \<Rightarrow> Normal (\<phi>arg v) | _ \<Rightarrow> Crash)}\<close>
+  unfolding Transition_of'_def \<phi>R_get_res'_def \<phi>R_get_res_entry'_def bind_def Return_def det_lift_def
+  by (cases ret; clarsimp simp add: set_eq_iff Id_on_iff split: option.split; blast)
+
+lemma getter_refinement:
+  \<open>Transition_of' (\<phi>R_get_res_entry' k) ret
+   \<r>\<e>\<f>\<i>\<n>\<e>\<s> Id_on ({1(k \<mapsto> any)} \<s>\<u>\<b>\<j> ret = Normal (\<phi>arg any))
+   \<w>.\<r>.\<t> basic_fiction \<i>\<n> {1(k \<mapsto> any)}\<close>
+  unfolding Fictional_Forward_Simulation_def getter_transition
+  apply (cases ret; clarsimp split: option.split simp add: basic_fiction_\<I> set_mult_expn Id_on_iff
+          Subjection_expn zero_set_def set_eq_iff prj.homo_mult times_fun)
+  by (smt (verit, best) domIff fun_1upd_homo fun_split_1_not_dom fun_upd_same map_upd_eqD1 sep_disj_partial_map_some_none sep_space_entry.sep_disj_get_name sep_space_entry_axioms)
+
+lemma getter_valid:
+  \<open>Valid_Proc (\<phi>R_get_res_entry' k)\<close>
+  unfolding Valid_Proc_def \<phi>R_get_res_entry'_def \<phi>R_get_res'_def bind_def Return_def det_lift_def
+  by (clarsimp split: option.split)
+
+
+subsubsection \<open>Setter\<close>
+
+lemma setter_refinement:
+  \<open>(\<forall>m. m \<in>\<^sub>S\<^sub>H domain \<longrightarrow> m k = Some any \<longrightarrow> m(k := u) \<in>\<^sub>S\<^sub>H domain)
+\<Longrightarrow> Transition_of' (\<phi>R_set_res' (\<lambda>f. f(k := u))) ret
+  \<r>\<e>\<f>\<i>\<n>\<e>\<s> pairself (fun_upd 1 k) ` {(Some any, u)} \<s>\<u>\<b>\<j> ret = Normal \<phi>V_none \<w>.\<r>.\<t> basic_fiction \<i>\<n> fun_upd 1 k ` {Some any}\<close>
+  apply (rule refinement_sub_fun[OF setter_transition[where F=\<open>\<lambda>f. f(k := u)\<close>]], assumption)
+  unfolding Fictional_Forward_Simulation_def setter_transition
+  apply (clarsimp simp add: basic_fiction_\<I> \<phi>expns prj.homo_mult times_fun_upd sep_disj_partial_map_upd
+        nonsepable_semigroup_sepdisj_fun SPACE_mult_homo \<r>_valid_split'
+        times_fun inj.homo_mult[symmetric] inject_wand_homo dom_mult)
+  subgoal premises prems for r R x' u' a
+  proof -
+    have t1[simp]: \<open>a ## 1(k \<mapsto> any)\<close>
+      using prems(5) prems(9) sep_disj_commuteI sep_disj_multD2 by blast
+    have t2[simp]: \<open>r ## (a * 1(k \<mapsto> any))\<close>
+      by (simp add: prems(5) prems(9) sep_disj_commuteI sep_disj_multI1 sep_mult_commute)
+    have t3[simp]: \<open>x' = clean u' * mk ((r * (a * 1(k \<mapsto> any)))(k := u)) \<and> ret = Normal \<phi>V_none\<close>
+      by (smt (z3) map_upd_Some_unfold prems(3) prems(5) sep_disj_partial_map_some_none t1 times_option(3))
+    have t4[simp]: \<open>mk ((r * (a * 1(k \<mapsto> any)))(k := u)) = mk (r * (a * 1(k := u)))\<close>
+      by (metis domIff fun_upd_same fun_upd_upd option.distinct(1) sep_disj_partial_map_upd t1 t2)
+    have t5[simp]: \<open>clean u' * mk a = u'\<close>
+      by (metis fun_split_1 prems(8))
+    show ?thesis
+      apply (simp add: prems, rule exI[where x=u']; simp add: prems; rule)
+      apply (smt (verit, ccfv_threshold) mk_homo_mult nonsepable_semigroup_sepdisj_fun prems(5) prems(9) sep_disj_clean sep_disj_mk sep_disj_multD1 sep_disj_multI1 sep_disj_multI2 sep_mult_assoc' sep_mult_left_commute t4 t5)
+      by (smt (verit, best) fun_1upd_homo_right1 fun_sep_disj_1_fupdt(1) inj.sep_disj_homo mult_1_class.mult_1_left nonsepable_semigroup_sepdisj_fun sep_disj_commute sep_disj_multD1 sep_disj_multI1 sep_mult_commute t1 t2 t5)
+  qed .
+
+
+end
+
+
+subsection \<open>Pointwise Base Fiction\<close>
+
+locale pointwise_base_fiction_for_partial_mapping_resource =
+   R: partial_map_resource Res
++  fiction_kind FIC.DOMAIN INTERPRET Fic \<open>R.basic_fiction o\<^sub>\<I> \<F>_pointwise I\<close>
+for Res :: "('key \<Rightarrow> 'val::nonsepable_semigroup option) resource_entry"
+and I :: \<open>('fic::sep_algebra, 'val option) interp\<close>
+and Fic :: "('key \<Rightarrow> 'fic) fiction_entry"
+begin
+
+sublocale fiction_base_for_mapping_resource Res \<open>\<F>_pointwise I\<close> Fic ..
+
+lemma "_getter_rule_2_":
+  \<open> refinement_projection I {x} \<subseteq> UNIV * {Some v}
+\<Longrightarrow> \<p>\<r>\<o>\<c> R.\<phi>R_get_res_entry' k \<lbrace> 1(k := x) \<Ztypecolon> \<phi> Identity \<longmapsto> \<lambda>ret. 1(k := x) \<Ztypecolon> \<phi> Identity \<s>\<u>\<b>\<j> ret = \<phi>arg v \<rbrace>\<close>
+  by (rule "__getter_rule__",
+      rule R.getter_valid,
+      rule sep_refinement_stepwise,
+      rule R.getter_refinement[THEN refinement_frame[where R=UNIV]],
+      unfold Subjection_Id_on Subjection_times,
+      rule refinement_subjection[OF constant_refinement],
+      rule \<F>_pointwise_projection[where D'=\<open>{x}\<close> and D=\<open>{Some v}\<close>, simplified],
+      assumption)
+
+lemma "_setter_rule_2_":
+  \<open> Id_on UNIV * {(Some v, u)} \<r>\<e>\<f>\<i>\<n>\<e>\<s> {(v', u')} \<w>.\<r>.\<t> I \<i>\<n> {v'}
+\<Longrightarrow> refinement_projection I {v'} \<subseteq> UNIV * {Some v}
+\<Longrightarrow> \<forall>m. m \<in>\<^sub>S\<^sub>H R.domain \<longrightarrow> m k = Some v \<longrightarrow> m(k := u) \<in>\<^sub>S\<^sub>H R.domain
+\<Longrightarrow> \<p>\<r>\<o>\<c> R.\<phi>R_set_res' (\<lambda>f. f(k := u))
+      \<lbrace> 1(k := v') \<Ztypecolon> \<phi> Identity \<longmapsto> 1(k := u') \<Ztypecolon> \<phi> Identity \<rbrace> \<close>
+  by (rule "__setter_rule__",
+      rule R.setter_valid,
+      rule sep_refinement_stepwise[
+        OF R.setter_refinement[THEN refinement_frame[where R=UNIV], unfolded Subjection_times]
+           refinement_subjection[OF \<F>_pointwise_refinement]
+           \<F>_pointwise_projection,
+         where D'1=\<open>{v'}\<close> and B4=\<open>{(v',u')}\<close>, simplified],
+      assumption,
+      assumption,
+      assumption)
+
+
+end
+
+
+subsection \<open>Pointwise Fiction\<close>
+
+locale pointwise_fiction_for_partial_mapping_resource =
+   R: partial_map_resource Res
++  fiction_kind FIC.DOMAIN INTERPRET Fic \<open>R.basic_fiction o\<^sub>\<I> \<F>_pointwise \<F>_it\<close>
+for Res :: "('key \<Rightarrow> 'val nosep option) resource_entry"
+and Fic :: "('key \<Rightarrow> 'val nosep option) fiction_entry"
+begin
+
+sublocale pointwise_base_fiction_for_partial_mapping_resource Res \<F>_it Fic ..
+
+lemmas setter_rule = "_setter_rule_2_"[OF \<F>_it_refinement \<F>_it_refinement_projection]
+lemmas getter_rule = "_getter_rule_2_"[OF \<F>_it_refinement_projection]
+lemmas allocate_rule = "__allocate_rule_2__"
+                            [OF \<F>_pointwise_refinement[OF \<F>_it_refinement, where u1=1, simplified]]
+
+end
+
+subsection \<open>Pointwise Share Fiction\<close>
+
+locale pointwise_share_fiction_for_partial_mapping_resource =
+   R: partial_map_resource Res
++  fiction_kind FIC.DOMAIN INTERPRET Fic \<open>R.basic_fiction o\<^sub>\<I> \<F>_pointwise (\<F>_functional to_share)\<close>
+for Res :: "('key \<Rightarrow> 'val nosep option) resource_entry"
+and Fic :: "('key \<Rightarrow> 'val nosep share option) fiction_entry"
+begin
+
+sublocale pointwise_base_fiction_for_partial_mapping_resource Res \<open>\<F>_functional to_share\<close> Fic ..
+
+lemmas setter_rule =
+  "_setter_rule_2_"[OF to_share.refinement[simplified], simplified,
+                    OF to_share.refinement_projection[where S=\<open>{Some v}\<close> and n = 1 for v, simplified]]
+
+lemmas getter_rule =
+  "_getter_rule_2_"[OF to_share.refinement_projection[where S=\<open>{x}\<close> for x, simplified], simplified]
+
+lemmas allocate_rule =
+  "__allocate_rule_2__"[OF \<F>_pointwise_refinement[OF to_share.refinement[where u=\<open>1\<close>, simplified], simplified],
+                        where u = \<open>Some u'\<close> for u', simplified]
+
+end
+
+
+
+section \<open>Two Level Parital Mapping\<close>
+
+subsection \<open>Preliminary\<close>
+
+definition \<open>map_fun_at g k f = (\<lambda>x. if x = k then g (f x) else f x)\<close>
+
+lemma map_fun_at_1[simp]: \<open>map_fun_at g k 1 = 1(k := g 1)\<close>
+  unfolding map_fun_at_def fun_eq_iff by simp
+
+lemma map_fun_at_const[simp]:
+  \<open>map_fun_at (\<lambda>_. u) k f = f(k := u)\<close>
+  unfolding map_fun_at_def fun_eq_iff by simp
+
+
+subsection \<open>Resource\<close>
+
+locale partial_map_resource2 =
+  mapping_resource Res
+for Res :: "('key \<Rightarrow> 'key2 \<Rightarrow> 'val::nonsepable_semigroup option) resource_entry"
+begin
+
+subsubsection \<open>Getter\<close>
+
+definition \<phi>R_get_res_entry' :: \<open>'key \<Rightarrow> 'key2 \<Rightarrow> 'val proc\<close>
+  where \<open>\<phi>R_get_res_entry' k k2 =
+    \<phi>R_get_res' \<bind> (\<lambda>res. case \<phi>arg.dest res k k2 of Some v \<Rightarrow> Return (\<phi>arg v) | _ \<Rightarrow> (\<lambda>_. {Invalid}))\<close>
+
+lemma getter_transition:
+  \<open> Transition_of' (\<phi>R_get_res_entry' k k2) ret
+        = Id_on {s. s \<in> SPACE \<and> ret = (case get s k k2 of Some v \<Rightarrow> Normal (\<phi>arg v) | _ \<Rightarrow> Crash)}\<close>
+  unfolding Transition_of'_def \<phi>R_get_res'_def \<phi>R_get_res_entry'_def bind_def Return_def det_lift_def
+  by (cases ret; clarsimp simp add: set_eq_iff Id_on_iff split: option.split; blast)
+
+lemma getter_refinement:
+  \<open>Transition_of' (\<phi>R_get_res_entry' k k2) ret
+   \<r>\<e>\<f>\<i>\<n>\<e>\<s> Id_on ({1(k := 1(k2 \<mapsto> any))} \<s>\<u>\<b>\<j> ret = Normal (\<phi>arg any))
+   \<w>.\<r>.\<t> basic_fiction \<i>\<n> {1(k := 1(k2 \<mapsto> any))}\<close>
+  unfolding Fictional_Forward_Simulation_def getter_transition
+  apply (cases ret; clarsimp split: option.split simp add: basic_fiction_\<I> set_mult_expn Id_on_iff
+          Subjection_expn zero_set_def set_eq_iff prj.homo_mult times_fun)
+  by (smt (verit, del_insts) fun_sep_disj_imply_v fun_upd_triv mult_1_class.mult_1_right option.exhaust option.inject sep_disj_commuteI sep_disj_get_name sep_disj_multD2 sep_disj_option_nonsepable(2) sep_mult_commute)
+
+lemma getter_valid:
+  \<open>Valid_Proc (\<phi>R_get_res_entry' k k2)\<close>
+  unfolding Valid_Proc_def \<phi>R_get_res_entry'_def \<phi>R_get_res'_def bind_def Return_def det_lift_def
+  by (clarsimp split: option.split)
+
+subsubsection \<open>Setter\<close>
+
+lemma setter_refinement:
+  \<open> \<forall>m. m \<in>\<^sub>S\<^sub>H domain \<longrightarrow> m k k2 = Some any \<longrightarrow> map_fun_at (map_fun_at (\<lambda>_. u) k2) k m \<in>\<^sub>S\<^sub>H domain
+\<Longrightarrow> Transition_of' (\<phi>R_set_res' (map_fun_at (map_fun_at (\<lambda>_. u) k2) k)) ret
+\<r>\<e>\<f>\<i>\<n>\<e>\<s> pairself (fun_upd 1 k) ` pairself (fun_upd 1 k2) ` {(Some any, u)} \<s>\<u>\<b>\<j> ret = Normal \<phi>V_none
+\<w>.\<r>.\<t> basic_fiction \<i>\<n> (fun_upd 1 k) ` (fun_upd 1 k2) ` {Some any}\<close>
+  apply (rule refinement_sub_fun[OF setter_transition[where F=\<open>map_fun_at (map_fun_at (\<lambda>_. u) k2) k\<close>]], assumption)
+  unfolding Fictional_Forward_Simulation_def setter_transition
+  apply (clarsimp simp add: basic_fiction_\<I> \<phi>expns prj.homo_mult times_fun_upd sep_disj_partial_map_upd
+        nonsepable_semigroup_sepdisj_fun SPACE_mult_homo \<r>_valid_split'
+        times_fun inj.homo_mult[symmetric] inject_wand_homo)
+  subgoal premises prems for r R x' u' a
+  proof -
+    have t1[simp]: \<open>a k k2 ## Some any\<close>
+      by (metis fun_sep_disj_imply_v fun_upd_triv prems(5) prems(9) sep_disj_commuteI sep_disj_multD2)
+    have t2[simp]: \<open>r k k2 ## a k k2 * Some any\<close>
+      by (metis fun_sep_disj_1_fupdt(1) fun_upd_triv nonsepable_semigroup_sepdisj_fun prems(5))
+    have t3[simp]: \<open>r k k2 * (a k k2 * Some any) = Some any\<close>
+      using t1 t2 by force
+    have t4[simp]: \<open>x' = clean u' * mk (map_fun_at (map_fun_at (\<lambda>_. u) k2) k (r * (a * 1(k := 1(k2 \<mapsto> any))))) \<and> ret = Normal \<phi>V_none\<close>
+      using prems(3) by fastforce
+    have t5[simp]: \<open>r ## 1(k := 1(k2 := u))\<close>
+      by (metis fun_sep_disj_1_fupdt(1) fun_upd_triv nonsepable_semigroup_sepdisj_fun prems(5))
+    have t6[simp]: \<open>(r * a) k k2 = None\<close>
+      by (metis sep_disj_multI1 sep_disj_option_nonsepable(1) t1 t2 times_fun)
+    then have [simp]:
+        \<open>map_fun_at (map_fun_at (\<lambda>_. u) k2) k (r * (a * 1(k := 1(k2 \<mapsto> any))))
+            = (r * a) * 1(k := 1(k2 := u))\<close>
+        unfolding map_fun_at_def fun_eq_iff times_fun_def
+        by simp
+    have t1[simp]: \<open>clean u' * mk a = u'\<close>
+      by (metis fun_split_1 prems(8))
+    show ?thesis
+      apply (simp, rule exI[where x=u']; simp add: prems; rule)
+      apply (smt (verit, del_insts) fun_sep_disj_1_fupdt(1) fun_upd_triv inj.homo_mult inj.sep_disj_homo_semi inject_assoc_homo nonsepable_semigroup_sepdisj_fun prems(5) prems(8) prems(9) sep_disj_multD1 sep_disj_multI1 sep_mult_commute sep_space_entry.times_fun_upd sep_space_entry_axioms times_fupdt_1_apply_sep)
+      by (metis (mono_tags, lifting) fun_sep_disj_1_fupdt(1) fun_upd_triv inj.sep_disj_homo_semi nonsepable_semigroup_sepdisj_fun prems(5) prems(8) prems(9) sep_disj_multD1 sep_disj_multI1 sep_disj_multI2)
+  qed .
+
+end
+
+
+subsection \<open>Pointwise Base Fiction\<close>
+
+locale pointwise_base_fiction_for_partial_mapping_resource2 =
+   R: partial_map_resource2 Res
++  fiction_kind FIC.DOMAIN INTERPRET Fic \<open>R.basic_fiction o\<^sub>\<I> \<F>_pointwise (\<F>_pointwise I)\<close>
+for Res :: "('key \<Rightarrow> 'key2 \<Rightarrow> 'val::nonsepable_semigroup option) resource_entry"
+and I :: \<open>('fic::sep_algebra, 'val option) interp\<close>
+and Fic :: "('key \<Rightarrow> 'key2 \<Rightarrow> 'fic) fiction_entry"
+begin
+
+sublocale fiction_base_for_mapping_resource Res \<open>\<F>_pointwise (\<F>_pointwise I)\<close> Fic ..
+
+lemma "_getter_rule_2_":
+  \<open> refinement_projection I {x} \<subseteq> UNIV * {Some v}
+\<Longrightarrow> \<p>\<r>\<o>\<c> R.\<phi>R_get_res_entry' k k2 \<lbrace> 1(k := 1(k2 := x)) \<Ztypecolon> \<phi> Identity \<longmapsto>
+                                    \<lambda>ret. 1(k := 1(k2 := x)) \<Ztypecolon> \<phi> Identity \<s>\<u>\<b>\<j> ret = \<phi>arg v \<rbrace>\<close>
+  by (rule "__getter_rule__",
+      rule R.getter_valid,
+      rule sep_refinement_stepwise,
+      rule R.getter_refinement[THEN refinement_frame[where R=UNIV]],
+      unfold Subjection_Id_on Subjection_times,
+      rule refinement_subjection[OF constant_refinement],
+      rule \<F>_pointwise_projection[where D'=\<open>{1(k2 := x)}\<close> and D=\<open>{1(k2 \<mapsto> v)}\<close>, simplified],
+      rule \<F>_pointwise_projection[where D'=\<open>{x}\<close> and D=\<open>{Some v}\<close>, simplified],
+      assumption)
+
+lemma "_setter_rule_2_":
+  \<open> Id_on UNIV * {(Some v, u)} \<r>\<e>\<f>\<i>\<n>\<e>\<s> {(v', u')} \<w>.\<r>.\<t> I \<i>\<n> {v'}
+\<Longrightarrow> refinement_projection I {v'} \<subseteq> UNIV * {Some v}
+\<Longrightarrow> \<forall>m. m \<in>\<^sub>S\<^sub>H R.domain \<longrightarrow> m k k2 = Some v \<longrightarrow> map_fun_at (map_fun_at (\<lambda>_. u) k2) k m \<in>\<^sub>S\<^sub>H R.domain
+\<Longrightarrow> \<p>\<r>\<o>\<c> R.\<phi>R_set_res' (map_fun_at (map_fun_at (\<lambda>_. u) k2) k)
+      \<lbrace> 1(k := 1(k2 := v')) \<Ztypecolon> \<phi> Identity \<longmapsto> 1(k := 1(k2 := u')) \<Ztypecolon> \<phi> Identity \<rbrace> \<close>
+  by (rule "__setter_rule__",
+      rule R.setter_valid,
+      rule sep_refinement_stepwise[
+        OF R.setter_refinement[THEN refinement_frame[where R=UNIV], unfolded Subjection_times]
+           refinement_subjection[OF \<F>_pointwise_refinement[OF \<F>_pointwise_refinement]]
+           \<F>_pointwise_projection[OF \<F>_pointwise_projection],
+        where D'2=\<open>{v'}\<close> and B6=\<open>{(v',u')}\<close>, simplified],
+      assumption,
+      assumption,
+      assumption)
+
+end
+
+subsection \<open>Pointwise Fiction\<close>
+
+locale pointwise_fiction_for_partial_mapping_resource2 =
+   R: partial_map_resource2 Res
++  fiction_kind FIC.DOMAIN INTERPRET Fic \<open>R.basic_fiction o\<^sub>\<I> \<F>_pointwise (\<F>_pointwise \<F>_it)\<close>
+for Res :: "('key \<Rightarrow> 'key2 \<Rightarrow> 'val nosep option) resource_entry"
+and Fic :: "('key \<Rightarrow> 'key2 \<Rightarrow> 'val nosep option) fiction_entry"
+begin
+
+sublocale pointwise_base_fiction_for_partial_mapping_resource2 Res \<F>_it Fic ..
+
+lemmas setter_rule = "_setter_rule_2_"[OF \<F>_it_refinement \<F>_it_refinement_projection]
+lemmas getter_rule = "_getter_rule_2_"[OF \<F>_it_refinement_projection]
+lemmas allocate_rule = "__allocate_rule_2__"[unfolded \<F>_pointwise_\<F>_it,
+                          OF \<F>_pointwise_refinement[OF \<F>_it_refinement, where u1=1, simplified, unfolded \<F>_pointwise_\<F>_it]]
+
+end
+
+
+subsection \<open>Pointwise Share Fiction\<close>
+
+locale pointwise_share_fiction_for_partial_mapping_resource2 =
+   R: partial_map_resource2 Res
++  fiction_kind FIC.DOMAIN INTERPRET Fic \<open>R.basic_fiction o\<^sub>\<I> \<F>_pointwise (\<F>_pointwise (\<F>_functional to_share))\<close>
+for Res :: "('key \<Rightarrow> 'key2 \<Rightarrow> 'val nosep option) resource_entry"
+and Fic :: "('key \<Rightarrow> 'key2 \<Rightarrow> 'val nosep share option) fiction_entry"
+begin
+
+sublocale pointwise_base_fiction_for_partial_mapping_resource2 Res \<open>\<F>_functional to_share\<close> Fic ..
+
+lemmas setter_rule =
+  "_setter_rule_2_""_setter_rule_2_"[OF to_share.refinement[simplified], simplified,
+                                     OF to_share.refinement_projection[where S=\<open>{Some v}\<close> and n = 1 for v, simplified]]
+lemmas getter_rule =
+  "_getter_rule_2_"[OF to_share.refinement_projection[where S=\<open>{x}\<close> for x, simplified], simplified]
+
+lemmas allocate_rule =
+  "__allocate_rule_2__"[OF \<F>_pointwise_refinement[OF pointwise_to_share.refinement[where u=\<open>1\<close>, simplified], simplified, unfolded to_share.\<F>_functional_pointwise]]
+
+end
+
+
+end
